constants and equations

code/theories/Ast.sig
@@ -1,26 +1,20 @@
-base : Type
 bool : Type
-type : Type
+const : Type
 term(tVar) : Type
 elim : Type
 
-TBase : base -> type
+tConst : const -> term
 
-TUnit : type
 tStar : term
 
-TProd : type -> type -> type
 tPair : term -> term -> term
 tProj : bool -> term -> term
 
-TFun : type -> type -> type
 tLam : (bind term in term) -> term
 tApp : term -> term -> term
 
-TEmp : type
 tAbort : term -> term
 
-TSum : type -> type -> type
 tIn : bool -> term -> term
 tIf : term -> (bind term in term) -> (bind term in term) -> term
 
