code/theories/BasicAst.v
@@ -1,12 +1,34 @@
 (** * Interpolation.BasicAst: parameters for the AST of terms *)
 
-Axiom base : Set.
-Axiom eqb_base : base -> base -> bool.
+Set Primitive Projections.
+
+Class Base : Type := {base : Set}.
+(* Axiom eqb_base : base -> base -> bool.
 Axiom eqb_base_refl : forall b, eqb_base b b = true.
-Axiom eqb_base_sound : forall b b', eqb_base b b' = true -> b = b'.
+Axiom eqb_base_sound : forall b b', eqb_base b b' = true -> b = b'. *)
+
+Inductive type `{b : Base} :=
+  | TBase : base -> type
+  | TUnit : type
+  | TProd : type -> type -> type
+  | TFun : type -> type -> type
+  | TEmp : type
+  | TSum : type -> type -> type.
+
+Class Lang `{ba : Base} : Type := {
+  const : Set ;
+  const_type : const -> type
+}.
+
+Definition EmptyLang `{b : Base} : Lang := {|
+  const := False ;
+  const_type := fun (e : False) => False_rec _ e
+|}.
 
 Inductive polarity := | pos | neg.
+
 Definition negp (p : polarity) := if p then neg else pos.
+
 Lemma negp_inv p : negp (negp p) = p.
 Proof.
   now destruct p.
