code/theories/Interpolation.v
@@ -1,519 +1,546 @@
-From Interpolation Require Import Utils Syntax Notations Reduction Typing Bidir MetaTheory.
 From Stdlib Require Import Relations Arith Lia Bool List RelationClasses.
+From Interpolation Require Import Utils Syntax Languages Notations Reduction Typing Bidir.
 
 (** ** Primitives for context splitting *)
 
-Inductive side : Set := | source | target.
+Section Splitting.
+  Context `{Lang}.
 
-Definition flip_side s := match s with | source => target | target => source end.
+  Inductive side : Set := | source | target.
 
-Inductive split : context -> context -> context -> Set :=
-  | split_emp : split ε ε ε
-  | split_s {Γ Γs Γt A} : split Γ Γs Γt -> split (Γ,,A) (Γs,,A) Γt
-  | split_t {Γ Γs Γt A} : split Γ Γs Γt -> split (Γ,,A) Γs (Γt,,A).
+  Definition flip_side s := match s with | source => target | target => source end.
 
-Fixpoint flip_split {Γ Γs Γt} (s : split Γ Γs Γt) : split Γ Γt Γs :=
-  match s with
-  | split_emp => split_emp
-  | split_s s => split_t (flip_split s)
-  | split_t s => split_s (flip_split s)
-  end.
+  Inductive split : context -> context -> context -> Set :=
+    | split_emp : split ε ε ε
+    | split_s {Γ Γs Γt A} : split Γ Γs Γt -> split (Γ,,A) (Γs,,A) Γt
+    | split_t {Γ Γs Γt A} : split Γ Γs Γt -> split (Γ,,A) Γs (Γt,,A).
 
-Fixpoint sren_s {Γ Γs Γt} (s : split Γ Γs Γt) : ren :=
-  match s with
-  | split_emp => id
-  | split_s s' => ⇑ (sren_s s')
-  | split_t s' => (sren_s s') >> ↑
-  end.
+  Fixpoint flip_split {Γ Γs Γt} (s : split Γ Γs Γt) : split Γ Γt Γs :=
+    match s with
+    | split_emp => split_emp
+    | split_s s => split_t (flip_split s)
+    | split_t s => split_s (flip_split s)
+    end.
 
-Fixpoint sren_t {Γ Γs Γt} (s : split Γ Γs Γt) : ren :=
-  match s with
-  | split_emp => id
-  | split_t s' => ⇑ (sren_t s')
-  | split_s s' => (sren_t s') >> ↑
-  end.
+  Fixpoint sren_s {Γ Γs Γt} (s : split Γ Γs Γt) : ren :=
+    match s with
+    | split_emp => id
+    | split_s s' => ⇑ (sren_s s')
+    | split_t s' => (sren_s s') >> ↑
+    end.
 
-Lemma flip_split_inv {Γ Γs Γt} (s : split Γ Γs Γt) :
-  flip_split (flip_split s) = s.
-Proof.
-  induction s ; cbn.
-  1: easy.
-  all: now rewrite IHs.
-Qed.
+  Fixpoint sren_t {Γ Γs Γt} (s : split Γ Γs Γt) : ren :=
+    match s with
+    | split_emp => id
+    | split_t s' => ⇑ (sren_t s')
+    | split_s s' => (sren_t s') >> ↑
+    end.
 
-Lemma sren_s_flip {Γ Γs Γt} (s : split Γ Γs Γt) :
-  sren_s (flip_split s) = sren_t s.
-Proof.
-  induction s ; cbn.
-  1: easy.
-  all: now rewrite IHs.
-Qed.
-
-Lemma sren_t_split {Γ Γs Γt} (s : split Γ Γs Γt) :
-  sren_t (flip_split s) = sren_s s.
-Proof.
-  rewrite <- (flip_split_inv s) at 2.
-  rewrite sren_s_flip.
-  reflexivity.
-Qed.
-
-Lemma sren_s_ty {Γ Γs Γt} (s : split Γ Γs Γt) :
-  Γ ⊢ (sren_s s) :: Γs.
-Proof.
-  induction s ; cbn.
-  all: eauto with typing.
-Qed.
-
-Lemma sren_t_ty {Γ Γs Γt} (s : split Γ Γs Γt) :
-  Γ ⊢ (sren_t s) :: Γt.
-Proof.
-  eapply ren_has_type_ext.
-  2: eapply sren_s_ty.
-  rewrite sren_s_flip.
-  reflexivity.
-Qed.
-
-Hint Resolve sren_s_ty sren_t_ty : typing.
-
-Fixpoint find_side {Γ Γs Γt} (s : split Γ Γs Γt) (n : nat) : option side :=
-  match s, n with
-  | split_emp, _ => None
-  | split_s _, 0 => Some source
-  | split_t _, 0 => Some target
-  | split_s s', S n' | split_t s', S n' => find_side s' n'
-  end.
-
-Lemma find_flip {Γ Γs Γt} (s : split Γ Γs Γt) (n : nat) :
-  find_side (flip_split s) n = option_map flip_side (find_side s n).
-Proof.
-  induction s in n |- * ; cbn ; try easy.
-  all: now destruct n ; cbn.
-Qed.
-
-Lemma in_context_find_none {Γ Γs Γt} (n : nat) (s : split Γ Γs Γt) T :
-  in_context n Γ T ->
-  find_side s n = None ->
-  False.
-Proof.
-  induction s in n |- * ; [|destruct n | destruct n] ; cbn.
-  - eauto with typing.
-  - congruence.
-  - intros Hin ?%IHs.
+  Lemma flip_split_inv {Γ Γs Γt} (s : split Γ Γs Γt) :
+    flip_split (flip_split s) = s.
+  Proof.
+    induction s ; cbn.
     1: easy.
-    exact Hin.
-  - congruence.
-  - intros Hin ?%IHs.
+    all: now rewrite IHs.
+  Qed.
+
+  Lemma sren_s_flip {Γ Γs Γt} (s : split Γ Γs Γt) :
+    sren_s (flip_split s) = sren_t s.
+  Proof.
+    induction s ; cbn.
     1: easy.
-    exact Hin.
-Qed.
+    all: now rewrite IHs.
+  Qed.
 
-Lemma find_side_some_l {Γ Γs Γt} (n : nat) (s : split Γ Γs Γt) :
-  find_side s n = Some source ->
-  {n' & {T & in_context n' Γs T /\ n = sren_s s n'}}.
-Proof.
-  intros Hside.
-  induction s in n, Hside |- * ; [|destruct n | destruct n] ; cbn in *.
-  - congruence.
-  - eexists 0, _ ; split ; reflexivity.
-  - edestruct IHs as (n'&e&[]) ; tea.
-    subst.
-    eexists (S n'),_ ; split ; cbn ; tea ; reflexivity.
-  - congruence.
-  - edestruct IHs as (n'&e&[]) ; tea.
-    subst.
-    eexists n',_ ; split ; cbn ; tea ; reflexivity.
-Qed.
+  Lemma sren_t_split {Γ Γs Γt} (s : split Γ Γs Γt) :
+    sren_t (flip_split s) = sren_s s.
+  Proof.
+    rewrite <- (flip_split_inv s) at 2.
+    rewrite sren_s_flip.
+    reflexivity.
+  Qed.
 
-Lemma find_side_some_r {Γ Γs Γt} (n : nat) (s : split Γ Γs Γt) :
-  find_side s n = Some target ->
-  {n' & {T & in_context n' Γt T /\ n = sren_t s n'}}.
-Proof.
-  intros e.
-  rewrite <- sren_s_flip.
-  apply find_side_some_l.
-  rewrite find_flip, e.
-  reflexivity.
-Qed.
+  Lemma sren_s_ty {Γ Γs Γt} (s : split Γ Γs Γt) :
+    Γ ⊢ (sren_s s) :: Γs.
+  Proof.
+    induction s ; cbn.
+    all: eauto with typing.
+  Qed.
 
-(** ** Atoms of a type/context *)
+  Lemma sren_t_ty {Γ Γs Γt} (s : split Γ Γs Γt) :
+    Γ ⊢ (sren_t s) :: Γt.
+  Proof.
+    eapply ren_typing_ext.
+    2: eapply sren_s_ty.
+    rewrite sren_s_flip.
+    reflexivity.
+  Qed.
 
-Fixpoint atoms_ty (p : polarity) (A : type) {struct A} : base -> Prop :=
-  match A with
-  | TBase b => if p then (sing b) else ∅
-  | TUnit | TEmp => ∅
-  | TFun A B => atoms_ty (negp p) A ∪ atoms_ty p B
-  | TProd A B | TSum A B => atoms_ty p A ∪ atoms_ty p B
-  end.
+  Hint Resolve sren_s_ty sren_t_ty : typing.
 
-Fixpoint atoms_ctx (p : polarity) (Γ : context) : base -> Prop :=
-  match Γ with
-  | nil => ∅
-  | cons A Γ => atoms_ctx p Γ ∪ (atoms_ty p A)
-  end.
+  Fixpoint find_side {Γ Γs Γt} (s : split Γ Γs Γt) (n : nat) : option side :=
+    match s, n with
+    | split_emp, _ => None
+    | split_s _, 0 => Some source
+    | split_t _, 0 => Some target
+    | split_s s', S n' | split_t s', S n' => find_side s' n'
+    end.
 
-Lemma atoms_in n Γ T :
-  in_context n Γ T ->
-  (forall p, atoms_ty p T ⊆ atoms_ctx p Γ).
-Proof.
-  intros H.
-  unfold in_context in *.
-  induction n in Γ, H |- * ; cbn.
-  - destruct Γ ; cbn in * ; [congruence|].
-    intros ? ? ?.
-    right.
-    now congruence.
-  - destruct Γ ; cbn in * ; [congruence|].
-    intros ? ? ?.
-    left.
-    now apply IHn.
-Qed.
+  Lemma find_flip {Γ Γs Γt} (s : split Γ Γs Γt) (n : nat) :
+    find_side (flip_split s) n = option_map flip_side (find_side s n).
+  Proof.
+    induction s in n |- * ; cbn ; try easy.
+    all: now destruct n ; cbn.
+  Qed.
+
+  Lemma in_context_find_none {Γ Γs Γt} (n : nat) (s : split Γ Γs Γt) T :
+    in_context n Γ T ->
+    find_side s n = None ->
+    False.
+  Proof.
+    induction s in n |- * ; [|destruct n | destruct n] ; cbn.
+    - eauto with typing.
+    - congruence.
+    - intros Hin ?%IHs.
+      1: easy.
+      exact Hin.
+    - congruence.
+    - intros Hin ?%IHs.
+      1: easy.
+      exact Hin.
+  Qed.
+
+  Lemma find_side_some_l {Γ Γs Γt} (n : nat) (s : split Γ Γs Γt) :
+    find_side s n = Some source ->
+    {n' & {T & in_context n' Γs T /\ n = sren_s s n'}}.
+  Proof.
+    intros Hside.
+    induction s in n, Hside |- * ; [|destruct n | destruct n] ; cbn in *.
+    - congruence.
+    - eexists 0, _ ; split ; reflexivity.
+    - edestruct IHs as (n'&e&[]) ; tea.
+      subst.
+      eexists (S n'),_ ; split ; cbn ; tea ; reflexivity.
+    - congruence.
+    - edestruct IHs as (n'&e&[]) ; tea.
+      subst.
+      eexists n',_ ; split ; cbn ; tea ; reflexivity.
+  Qed.
+
+  Lemma find_side_some_r {Γ Γs Γt} (n : nat) (s : split Γ Γs Γt) :
+    find_side s n = Some target ->
+    {n' & {T & in_context n' Γt T /\ n = sren_t s n'}}.
+  Proof.
+    intros e.
+    rewrite <- sren_s_flip.
+    apply find_side_some_l.
+    rewrite find_flip, e.
+    reflexivity.
+  Qed.
+
+End Splitting.
 
 Section Interpolation.
+  Context `{Lang}.
 
-(** With the splitting of the context given by Γs and Γt and the type A,
-  I is a valid interpolating type. *)
-Definition interpolate_ty Γs Γt A M :=
-  forall p, atoms_ty p M ⊆ (atoms_ctx p Γs) ∩ (atoms_ctx (negp p) Γt ∪ atoms_ty p A).
+  (** With the splitting of the context given by Γs and Γt and the type A,
+    I is a valid interpolating type. *)
+  Definition interpolate_ty Γs Γt A M (c : const_split): Prop :=
+    forall p, atoms_ty p M ⊆ 
+      (atoms_ctx p Γs ∪ atoms_const p c.(pconst_l)) ∩
+      (atoms_ctx (negp p) Γt ∪ (atoms_const (negp p) c.(pconst_r)) ∪ atoms_ty p A).
 
-Definition interpolate_tm {Γ Γs Γt} (s : split Γ Γs Γt) M A t l r :=
-  (Γs ⊢ l :: M) /\ (Γt ,, M ⊢ r :: A) /\
-  r⟨⇑ (sren_t s)⟩[l⟨sren_s s⟩..] ⤳* t.
+  Definition interpolate_tm {Γ Γs Γt} (s : split Γ Γs Γt) (c : const_split) M A t l r :=
+    (Γs ⊢ l :: M) /\ (atoms_tm l ⊆ c.(pconst_l)) /\
+    (Γt ,, M ⊢ r :: A) /\ (atoms_tm r ⊆ c.(pconst_r)) /\
+    r⟨⇑ (sren_t s)⟩[l⟨sren_s s⟩..] ⤳* t.
 
-Let Pcheck Γ T t := forall Γs Γt (s : split Γ Γs Γt),
-  exists M l r,
-    interpolate_ty Γs Γt T M /\ interpolate_tm s M T t l r.
+  Let Pcheck Γ T t := forall Γs Γt (s : split Γ Γs Γt) (c : const_split),
+    exists M l r,
+      interpolate_ty Γs Γt T M c /\ interpolate_tm s c M T t l r.
 
-Let Pinf Γ T t := forall Γs Γt (s : split Γ Γs Γt),
-  (
-    (forall p, atoms_ty p T ⊆ atoms_ctx p Γt) /\
-    (exists M l r, 
-      (forall p, atoms_ty p M ⊆ (atoms_ctx p Γs) ∩ (atoms_ctx (negp p) Γt)) /\
-      interpolate_tm s M T t l r)
-  ) \/ (
-    (forall p, atoms_ty p T ⊆ atoms_ctx p Γs) /\
-    (exists M l r, 
-      (forall p, atoms_ty p M ⊆ (atoms_ctx (negp p) Γs) ∩ (atoms_ctx p Γt)) /\
-      interpolate_tm (flip_split s) M T t l r)
-  ).
+  Let Pinf Γ T t := forall Γs Γt (s : split Γ Γs Γt) (c : const_split),
+    (
+      (forall p, atoms_ty p T ⊆ atoms_ctx p Γt ∪ atoms_const p c.(pconst_r)) /\
+      (exists M l r, 
+        (forall p, atoms_ty p M ⊆ (atoms_ctx p Γs ∪ atoms_const p c.(pconst_l))
+                                  ∩ (atoms_ctx (negp p) Γt ∪ atoms_const (negp p) c.(pconst_r)))
+        /\ interpolate_tm s c M T t l r)
+    ) \/ (
+      (forall p, atoms_ty p T ⊆ atoms_ctx p Γs ∪ atoms_const p c.(pconst_l)) /\
+      (exists M l r, 
+        (forall p, atoms_ty p M ⊆ (atoms_ctx (negp p) Γs ∪ atoms_const (negp p) c.(pconst_l))
+                                  ∩ (atoms_ctx p Γt ∪ atoms_const p c.(pconst_r)))
+        /\ interpolate_tm (flip_split s) (flip_csplit c) M T t l r)
+    ).
 
-Theorem interpolation_ind : bidir_concl Pcheck Pinf.
-Proof.
-  apply bidir_ind.
-  - (* case tStar *)
-    intros Γ Γs Γt s.
-    exists TUnit, tStar, tStar.
-    split.
-    + unfold interpolate_ty.
-      intros ; cbn.
-      intros ? [].
-    + red.
+  Ltac pre_crush_incl :=
+    unfold interpolate_ty in * ;
+    intros ;
+    repeat match goal with
+      | b : polarity |- _ => destruct b
+      | H : forall b : polarity, _ |- _ => pose proof (H pos) ; pose proof (H neg) ; cbn in * ; clear H
+    end.
+
+  Ltac crush_incl := pre_crush_incl ; set_solver.
+
+  Theorem interpolation_ind : bidir_concl Pcheck Pinf.
+  Proof.
+    apply bidir_ind ; subst Pcheck Pinf.
+
+    - (* case tStar *)
+      intros Γ Γs Γt s.
+      exists TUnit, tStar, tStar.
+      split.
+      1: solve [crush_incl].
+      red.
       prod_splitter.
-      1-2: now auto with typing.
+      1,3: now auto with typing.
+      1,2: solve [crush_incl].
       reflexivity.
-  - (* case tLam *)
-    intros Γ A B t _ IH Γs Γt s.
-    destruct (IH Γs (Γt,,A) (split_t s)) as (M&l&r&HM&Ht).
-    exists M, l, (tLam (r⟨swap_var⟩)).
-    split.
-    + intros p b Hb.
-      specialize (HM p b Hb).
-      now cbn in *.
-    + unfold interpolate_tm in * ; cbn in *.
-      destruct Ht as (?&?&e).
+
+    - (* case tLam *)
+      intros Γ A B t _ IH Γs Γt s c.
+      destruct (IH Γs (Γt,,A) (split_t s) c) as (M&l&r&HM&Ht).
+      exists M, l, (tLam (r⟨swap_var⟩)).
+      split.
+      1: clear -HM ; solve [crush_incl].
+      
+      unfold interpolate_tm in * ; cbn in *.
+      destruct Ht as (?&?&?&?&e).
       prod_splitter.
-      1-2: now eauto with typing.
+      1,3: now eauto with typing.
+      1: solve [crush_incl].
+      1: rewrite atoms_ren ; solve [crush_incl].
+
       refold.
-      rewrite swap_shift2, swap_shift1, <- e.
-      apply ereflexivity.
-      now asimpl.
-  - (* case tPair *)
-    intros Γ A B t t' _ IHA _ IHB Γs Γt s.
-    destruct (IHA Γs Γt s) as (M & l & r & HM & (?&?&et)).
-    destruct (IHB Γs Γt s) as (M' & l' & r' & HM' & (?&?&et')).
-    exists (TProd M M'), (tPair l l'),
-      (tPair (r[tip tFst]) (r'[tip tSnd])).
-    split.
-    + intros p b [Hb|Hb'].
-      1: specialize (HM p b Hb).
-      2: specialize (HM' p b Hb').
-      all: now cbn in *.
-    + unfold interpolate_tm in * ; cbn in *.
-      prod_splitter.
-      1-2: now eauto 20 with typing.
-      now rewrite !tip_shift, !tip_subst, ST_Fst, ST_Snd, et, et'.
-  - (* case tLeft *)
-    intros * _ IH ?? s.
-    destruct (IH _ _ s) as (M & l & r & HM & Ht).
-    exists M, l, (tLeft r).
-    split.
-    + intros ?? Hb.
-      specialize (HM _ _ Hb).
-      now cbn in *.
-    + unfold interpolate_tm in * ; cbn in *.
-      destruct Ht as (?&?&e).
-      prod_splitter.
-      1-2: eauto with typing.
-      now rewrite e.
-  - (* case tRight *)
-    intros * _ IH ?? s.
-    destruct (IH _ _ s) as (M & l & r & HM & Ht).
-    exists M, l, (tRight r).
-    split.
-    + intros ?? Hb.
-      specialize (HM _ _ Hb).
-      now cbn in *.
-    + unfold interpolate_tm in * ; cbn in *.
-      destruct Ht as (?&?&e).
-      prod_splitter.
-      1-2: eauto with typing.
-      now rewrite e.
-  - (* case tAbort *)
-    intros * _ IH ?? s.
-    destruct (IH _ _ s) as [[_ (M&l&r&[HM (?&?&e)])]|[_ (M&l&r&[HM (?&?&e)])]] ; tea.
-    + exists M, l, (tAbort r).
+      now rewrite swap_up2, swap_up1, renRen_term, e.
+    
+    - (* case tPair *)
+      intros Γ A B t t' _ IHA _ IHB Γs Γt s c.
+      destruct (IHA Γs Γt s c) as (M & l & r & HM & (?&?&?&?&et)).
+      destruct (IHB Γs Γt s c) as (M' & l' & r' & HM' & (?&?&?&?&et')).
+      exists (TProd M M'), (tPair l l'),
+        (tPair (r[tip tFst]) (r'[tip tSnd])).
       split.
-      * intros ?? Hb.
-        specialize (HM _ _ Hb).
-        now cbn in *.
-      * unfold interpolate_tm in * ; cbn in *.
+      1: clear -HM HM' ; solve [crush_incl].
+      
+      unfold interpolate_tm in * ; cbn in *.
+      prod_splitter.
+      1,3: now eauto 20 with typing.
+      1: solve [crush_incl].
+      + erewrite union_mono.
+        2-3: rewrite atoms_tm_subst, atoms_subst_tip ; cbn ; reflexivity.
+        set_solver.
+      
+      + now rewrite !tip_up_ren, !tip_subst, ST_Fst, ST_Snd, et, et'.
+    
+      - (* case tLeft *)
+      intros * _ IH ?? s c.
+      destruct (IH _ _ s c) as (M & l & r & HM & Ht).
+      exists M, l, (tLeft r).
+      split.
+      1: clear -HM ; solve [crush_incl].
+      
+      unfold interpolate_tm in * ; cbn in *.
+      destruct Ht as (?&?&?&?&e).
+      prod_splitter.
+      1,3: eauto with typing.
+      1-2: solve [crush_incl].
+      now rewrite e.
+    
+    - (* case tRight *)
+      intros * _ IH ?? s c.
+      destruct (IH _ _ s c) as (M & l & r & HM & Ht).
+      exists M, l, (tRight r).
+      split.
+      1: clear -HM ; solve [crush_incl].
+
+      unfold interpolate_tm in * ; cbn in *.
+      destruct Ht as (?&?&?&?&e).
+      prod_splitter.
+      1,3: eauto with typing.
+      1-2: solve [crush_incl].
+      now rewrite e.
+    
+      - (* case tAbort *)
+      intros * _ IH ?? s c.
+      destruct (IH _ _ s c) as [[_ (M&l&r&[HM (?&?&?&?&e)])]|[_ (M&l&r&[HM (?&?&?&?&e)])]] ; tea.
+
+      + exists M, l, (tAbort r).
+        split.
+        1: clear -HM ; solve [crush_incl].
+
+        unfold interpolate_tm in * ; cbn in *.
         prod_splitter.
-        1-2: eauto with typing.
+        1,3: eauto with typing.
+        1-2: solve [crush_incl].
         now rewrite e.
-    + exists (TFun M TEmp), (tLam r), (tAbort (tApp (tVar 0) l⟨↑⟩)).
-      split.
-      * intros p b [[HΓ%HM Hb]%dup|] ; cbn in * ; [|easy].
-        now rewrite negp_inv in HΓ.
-      * unfold interpolate_tm in *.
+
+      + exists (TFun M TEmp), (tLam r), (tAbort (tApp (tVar 0) l⟨↑⟩)).
+        split.
+        1: clear -HM ; solve [crush_incl].
+
+        unfold interpolate_tm in *.
         prod_splitter.
-        1-2: eauto 20 with typing.
-        cbn.
-        rewrite ST_Beta_Fun, <- e.
+        1,3: eauto 20 with typing.
+        1: cbn in * ; solve [crush_incl].
+        1: cbn in * ; rewrite atoms_ren ; solve [crush_incl].
+
+        cbn ; refold.
+        rewrite ST_Beta_Fun.
+        rewrite sren_s_flip, sren_t_split in e.
+        apply R_Abort_cong.
+        etransitivity ; [|eassumption].
         apply ereflexivity.
-        rewrite sren_s_flip, sren_t_split.
         substify.
         now asimpl.
-  - (* case tIf *)
-    intros Γ A B T s bl br ? IHs ? IHl ? IHr ?? sp.
-    destruct (IHs _ _ sp) as [[HMsum (M&l&r&[HMs (?&?&es)])]|[HMsum (M&l&r&[HMs (?&?&es)])]] ; tea.
-    + destruct (IHl _ _ (split_t sp)) as (Ml & ll & rl & HMl & (?&?&etl)).
-      destruct (IHr _ _ (split_t sp)) as (Mr & lr & rr & HMr & (?&?&etr)).
+
+    - (* case tIf *)
+      intros Γ A B T s bl br ? IHs ? IHl ? IHr ?? sp c.
+      destruct (IHs _ _ sp c) as [[HMsum (M&l&r&[HMs (?&?&?&?&es)])]|[HMsum (M&l&r&[HMs (?&?&?&?&es)])]] ; tea.
+
+      + destruct (IHl _ _ (split_t sp) c) as (Ml & ll & rl & HMl & (?&?&?&?&etl)).
+        destruct (IHr _ _ (split_t sp) c) as (Mr & lr & rr & HMr & (?&?&?&?&etr)).
+        exists (TProd M (TProd Ml Mr)), (tPair l (tPair ll lr)),
+          ((tIf r[tip tFst]
+            rl[(tip (fun x => (tFst (tSnd x))))]⟨swap_var⟩
+            rr[(tip (fun x => tSnd (tSnd x)))]⟨swap_var⟩)).
+        split.
+        1: clear -HMsum HMs HMl HMr ; solve [crush_incl].
+
+        unfold interpolate_tm in *.
+        prod_splitter.
+        1,3: eauto 20 with typing.
+        1: solve [crush_incl].
+        * cbn.
+          etransitivity.
+          1: repeat apply union_mono ; rewrite ?atoms_ren, atoms_tm_subst, atoms_subst_tip ; cbn ; reflexivity.
+          set_solver.
+
+        * cbn ; refold.
+          rewrite !swap_up2, !swap_up1, !tip_up_ren, !tip_subst ; cbn ; try easy.
+          now rewrite !ST_Snd, !ST_Fst, renRen_term, renRen_term, etl, etr, es.
+
+      + rewrite sren_s_flip, sren_t_split in es.
+        destruct (IHl _ _ (split_s sp) c) as (Ml & ll & rl & HMl & (?&?&?&?&etl)).
+        destruct (IHr _ _ (split_s sp) c) as (Mr & lr & rr & HMr & (?&?&?&?&etr)).
+        exists (TFun M (TSum Ml Mr)),
+          (tLam (tIf r (tLeft ll⟨↑⟩⟨swap_var⟩) (tRight lr⟨↑⟩⟨swap_var⟩))),
+          (tIf (tApp (tVar 0) l⟨↑⟩) rl⟨↑⟩⟨swap_var⟩ rr⟨↑⟩⟨swap_var⟩).
+        split.
+        1: clear -HMsum HMs HMl HMr ; solve [crush_incl].
+
       unfold interpolate_tm in *.
-      exists (TProd M (TProd Ml Mr)), (tPair l (tPair ll lr)),
-        ((tIf r[tip tFst]
-          rl[(tip (fun x => (tFst (tSnd x))))]⟨swap_var⟩
-          rr[(tip (fun x => tSnd (tSnd x)))]⟨swap_var⟩)).
-      split.
-      * intros p x Hp.
-        specialize (HMsum (negp p) x).
-        specialize (HMs p x).
-        specialize (HMl p x).
-        specialize (HMr p x).
-        now cbn in *.
-      * prod_splitter.
-        1-2: now eauto 20 with typing.
-        cbn ; refold.
-        rewrite !swap_shift2, !swap_shift1, !tip_shift, !tip_subst ; cbn ; try easy.
-        now rewrite !ST_Snd, !ST_Fst, !renRen_term, etl, etr, es.
-    + rewrite sren_s_flip, sren_t_split in es.
-      destruct (IHl _ _ (split_s sp)) as (Ml & ll & rl & HMl & (?&?&etl)).
-      destruct (IHr _ _ (split_s sp)) as (Mr & lr & rr & HMr & (?&?&etr)).
-      unfold interpolate_tm in *.
-      exists (TFun M (TSum Ml Mr)),
-        (tLam (tIf r (tLeft ll⟨↑⟩⟨swap_var⟩) (tRight lr⟨↑⟩⟨swap_var⟩))),
-        (tIf (tApp (tVar 0) l⟨↑⟩) rl⟨↑⟩⟨swap_var⟩ rr⟨↑⟩⟨swap_var⟩).
-      split.
-      * intros p x Hp.
-        clear -HMsum HMs HMl HMr Hp.
-        unfold interpolate_ty in *.
-        cbn in *.
-        specialize (HMsum p x).
-        specialize (HMs (negp p) x).
-        rewrite negp_inv in HMs.
-        specialize (HMl p x).
-        specialize (HMr p x).
-        now cbn in *.
-      * prod_splitter.
-        1-2: now eauto 20 with typing.
-        cbn ; refold.
+      prod_splitter.
+      1,3: now eauto 20 with typing.
+      * cbn.
+        etransitivity.
+        1: repeat apply union_mono ; rewrite ?atoms_ren ; reflexivity.
+        set_solver.
+      * cbn.
+        etransitivity.
+        1: repeat apply union_mono ; rewrite ?atoms_ren ; reflexivity.
+        set_solver.
+      
+      * cbn ; refold.
         clear -es etl etr.
-        rewrite !swap_shift2, !swap_shift1, !ST_Beta_Fun.
-        cbn.
-        rewrite ST_If_If, !ST_Left, !ST_Right, !swap_shift2, !swap_shift1 ; refold.
+        rewrite !swap_up2, !swap_up1, !ST_Beta_Fun.
+        cbn ; refold.
+        rewrite ST_If_If, !ST_Left, !ST_Right, !swap_up2, !swap_up1 ; refold.
         apply R_If_cong.
         all: etransitivity ; [|eassumption].
         all: apply ereflexivity.
-        ++ now substify ; asimpl.
-        ++ cbn.
-          rewrite !renRen_term ; refold.
-          apply subst_term_morphism.
-          ** intros [|] ; cbn ; [|easy].
-              now substify ; asimpl. 
-          ** now substify ; asimpl.
-        ++ cbn.
-          rewrite !renRen_term ; refold.
-          apply subst_term_morphism.
-          ** intros [|] ; cbn ; [|easy].
-              now substify ; asimpl. 
-          ** now substify ; asimpl.
-  - (* case demote *)
-    intros * _ IH -> ?? s.
-    destruct (IH _ _ s) as [[? (M&l&r&[HM ?])]|[Hat (M&l&r&[HM (?&?&erl)])]] ; tea.
-    + exists M, l, r ; split.
-      2: easy.
-      intros p b [?%HM Hb]%dup ; cbn in * ; easy.
-    + exists (TFun M A), (tLam r), (tApp (tVar 0) l⟨↑⟩).
-      split.
-      * intros p b [[HΓ%HM Hb]%dup| HA] ; cbn in *.
-        1: rewrite negp_inv in HΓ ; easy.
-        split ; [|easy].
-        now apply Hat.
-      * unfold interpolate_tm in *.
+        -- now substify ; asimpl.
+        -- cbn.
+           rewrite !renRen_term ; refold.
+           apply subst_term_morphism.
+           2: now substify ; asimpl.
+           intros [|] ; cbn ; [|easy].
+           now substify ; asimpl.
+        -- cbn.
+           rewrite !renRen_term ; refold.
+           apply subst_term_morphism.
+           2: now substify ; asimpl.
+           intros [|] ; cbn ; [|easy].
+           now substify ; asimpl.
+
+    - (* case demote *)
+      intros * _ IH -> ?? s c.
+      destruct (IH _ _ s c) as [[? (M&l&r&[HM ?])]|[Hat (M&l&r&[HM (?&?&?&?&erl)])]] ; tea.
+
+      + exists M, l, r ; split.
+        1: clear -HM ; solve [crush_incl].
+        easy.
+      + exists (TFun M A), (tLam r), (tApp (tVar 0) l⟨↑⟩).
+        split.
+        1: clear -HM Hat ; solve [crush_incl].
+
+        unfold interpolate_tm in *.
         prod_splitter.
-        1-2: now eauto 20 with typing.
+        1,3: now eauto 20 with typing.
+        1: solve [crush_incl].
+        1: cbn ; rewrite atoms_ren ; set_solver.
         cbn.
         rewrite ST_Beta_Fun, <- erl.
         apply ereflexivity.
         rewrite sren_s_flip, sren_t_split.
         substify.
         now asimpl.
-  - (* case tVar *)
-    intros ? n T Hin ?? s.
-    destruct (find_side s n) as [[]|] eqn:e.
-    3: exfalso ; now eauto using in_context_find_none.
-    + right.
-      apply find_side_some_l in e as (n'&A&[? ->]).
-      eapply in_context_inj in Hin.
-      2:now eapply sren_s_ty.
-      subst.
-      split.
-      1: now eapply atoms_in.
-      exists TUnit, tStar, (tVar (S n')).
-      split.
-      1: intros ? ? ? ; now cbn in *.
-      unfold interpolate_tm.
-      prod_splitter.
-      1-2: eauto with typing.
-      cbn.
-      now rewrite sren_t_split.
-    + left.
-      apply find_side_some_r in e as (n'&A&[? ->]).
-      eapply in_context_inj in Hin.
-      2:now eapply sren_t_ty.
-      subst.
-      split.
-      1: now eapply atoms_in.
-      exists TUnit, tStar, (tVar (S n')).
-      split.
-      1: intros ? ? ? ; now cbn in *.
-      unfold interpolate_tm.
-      prod_splitter.
-      1-2: eauto with typing.
-      reflexivity.
-  - (* case tApp *)
-    intros Γ A B n u _ Hn _ IHu Γs Γt s.
-    destruct (Hn _ _ s) as
-      [[IHpol (Mt&lt&rt&(IHt&?&?&et))]|[IHpol (Mt&lt&rt&(IHt&?&?&et))]].
-    + left.
-      cbn in *.
-      specialize (IHu _ _ s) as (Mu&lu&ru&(IHMu&?&?&eu)).
-      split.
-      1: now intros ?? Hb ; eapply IHpol ; cbn.
-      exists (TProd Mt Mu), (tPair lt lu),
-        (tApp (rt[tip tFst]) (ru[(tip tSnd)])).
-      cbn.
-      split.
-      * intros ? b ? ; cbn in *.
-        specialize (IHt p b).
-        specialize (IHMu p b).
-        specialize (IHpol (negp p) b).
-        rewrite negp_inv in IHpol.
-        cbn in *.
-        easy.
-      * unfold interpolate_tm in *.
+
+    - (* case tVar *)
+      intros ? n T Hin ?? s c.
+      destruct (find_side s n) as [[]|] eqn:e.
+      3: exfalso ; now eauto using in_context_find_none.
+
+      + right.
+        apply find_side_some_l in e as (n'&A&[? ->]).
+        eapply in_context_inj in Hin.
+        2:now eapply sren_s_ty.
+        subst.
+        split.
+        1: intros ; rewrite atoms_in ; tea ; set_solver.
+
+        exists TUnit, tStar, (tVar (S n')).
+        split.
+        1: intros ; cbn ; set_solver.
+        unfold interpolate_tm.
         prod_splitter.
-        1-2: now eauto 20 with typing.
+        1,3: eauto with typing.
+        1-2: solve [crush_incl].
         cbn.
-        now rewrite !tip_shift, !tip_subst, ST_Fst, ST_Snd, eu, et.
-    + right.
-      cbn in *.
-      specialize (IHu _ _ (flip_split s)) as (Mu&lu&ru&(IHMu&?&?&eu)).
-      split.
-      1: now intros ?? Hb ; eapply IHpol ; cbn.
-      exists (TProd Mt Mu), (tPair lt lu),
-        (tApp (rt[tip tFst]) (ru[tip tSnd])).
-      cbn.
-      split.
-      * intros ? b ? ; cbn in *.
-        specialize (IHt p b).
-        specialize (IHMu p b).
-        specialize (IHpol (negp p) b).
-        rewrite negp_inv in IHpol.
-        cbn in *.
-        easy.
-      * unfold interpolate_tm in *.
+        now rewrite sren_t_split.
+
+      + left.
+        apply find_side_some_r in e as (n'&A&[? ->]).
+        eapply in_context_inj in Hin.
+        2:now eapply sren_t_ty.
+        subst.
+        split.
+        1: intros ; rewrite atoms_in ; tea ; set_solver.
+
+        exists TUnit, tStar, (tVar (S n')).
+        split.
+        1: solve [crush_incl].
+
+        unfold interpolate_tm.
         prod_splitter.
-        1-2: now eauto 20 with typing.
+        1,3: eauto with typing.
+        1-2: solve [crush_incl].
+        reflexivity. 
+
+    - (* case tConst *)
+      intros Γ c ?? ? csplit.
+      destruct (const_cover csplit c).
+      
+      + right.
+        split.
+        1: now right ; eexists.
+
+        exists TUnit, tStar, (tConst c).
+        split.
+        1: solve [crush_incl].
+        red ; prod_splitter.
+        1,3: now eauto with typing.
+        1-2: crush_incl.
+
+        reflexivity.
+      
+      + left.
+        split.
+        1: now right ; eexists.
+
+        exists TUnit, tStar, (tConst c).
+        split.
+        1: solve [crush_incl].
+        red ; prod_splitter.
+        1,3: now eauto with typing.
+        1-2: crush_incl.
+
+        reflexivity.
+
+    - (* case tApp *)
+      intros Γ A B n u _ Hn _ IHu Γs Γt s c.
+      destruct (Hn _ _ s c) as
+        [[IHpol (Mt&lt&rt&(IHt&?&?&?&?&et))]|[IHpol (Mt&lt&rt&(IHt&?&?&?&?&et))]].
+
+      + left.
+        cbn in *.
+        specialize (IHu _ _ s c) as (Mu&lu&ru&(IHMu&?&?&?&?&eu)).
+        split.
+        1: clear -IHpol IHt IHMu ; solve [crush_incl].
+        exists (TProd Mt Mu), (tPair lt lu),
+          (tApp (rt[tip tFst]) (ru[(tip tSnd)])).
         cbn.
-        now rewrite !tip_shift, !tip_subst, ST_Fst, ST_Snd, eu, et.
-  - (* case tProj *)
-    intros * _ IH Γs Γt s.
-    destruct (IH _ _ s) as [[IHb (M&l&r&(?&?&?&etm))]|[IHb (M&l&r&(?&?&?&etm))]].
-    + left.
-      split.
-      * intros p.
-        destruct b.
-        all: intros b Hb ; apply IHb.
-        all: now cbn.
-      * exists M, l, (tProj b r).
-        split ; [easy|].
+        split.
+        1: clear -IHpol IHt IHMu ; solve [crush_incl].
+
+        unfold interpolate_tm in *.
+        prod_splitter.
+        1,3: now eauto 20 with typing.
+        1: solve [crush_incl].
+        1:{
+          cbn.
+          erewrite union_mono.
+          2,3: rewrite atoms_tm_subst, atoms_subst_tip ; cbn ; reflexivity.
+          set_solver.
+        }
+        cbn.
+        now rewrite !tip_up_ren, !tip_subst, ST_Fst, ST_Snd, eu, et.
+
+      + right.
+        cbn in *.
+        specialize (IHu _ _ (flip_split s) (flip_csplit c)) as (Mu&lu&ru&(IHMu&?&?&?&?&eu)).
+        split.
+        1: clear -IHpol IHt IHMu ; solve [crush_incl].
+        exists (TProd Mt Mu), (tPair lt lu),
+          (tApp (rt[tip tFst]) (ru[tip tSnd])).
+        cbn.
+        split.
+        1: clear -IHpol IHt IHMu; solve [crush_incl].
+        
+        unfold interpolate_tm in *.
+        prod_splitter.
+        1,3: now eauto 20 with typing.
+        1: solve [crush_incl].
+        1:{
+          cbn.
+          erewrite union_mono.
+          2,3: rewrite atoms_tm_subst, atoms_subst_tip ; cbn ; reflexivity.
+          set_solver.
+        }
+        cbn.
+        now rewrite !tip_up_ren, !tip_subst, ST_Fst, ST_Snd, eu, et.
+
+    - (* case tProj *)
+      intros * _ IH Γs Γt s c.
+      destruct (IH _ _ s c) as [[IHb (M&l&r&(HM&?&?&?&?&etm))]|[IHb (M&l&r&(HM&?&?&?&?&etm))]].
+      + left.
+        split.
+        1: destruct b ; clear -HM IHb ; solve [crush_incl].
+        exists M, l, (tProj b r).
+        split.
+        1: solve [crush_incl].
+
         unfold interpolate_tm in * ; prod_splitter.
-        2: destruct b.
-        1-3: now eauto with typing.
+        3: destruct b.
+        1,3,4: now eauto with typing.
+        1-2: easy.
         cbn.
         now rewrite etm.
-    + right.
-      split.
-      * intros p.
-        destruct b.
-        all: intros b Hb ; apply IHb.
-        all: now cbn.
-      * exists M, l, (tProj b r).
+      
+      + right.
+        split.
+        1: destruct b ; clear -HM IHb ; solve [crush_incl].
+
+        exists M, l, (tProj b r).
         split ; [easy|].
         unfold interpolate_tm in * ; prod_splitter.
-        2: destruct b ; cbn.
-        1-3: now eauto with typing.
+        3: destruct b ; cbn.
+        1,3,4: now eauto with typing.
+        1-2: easy.
         cbn.
         now rewrite etm.
-Qed.
+  Qed.
 
 End Interpolation.
-
-
-Corollary interpolation (A C : type) (t : term) :
-  (ε,,A ⊢ t :: C) ->
-  exists B u r l,
-    (forall p, atoms_ty p B ⊆ (atoms_ty p A) ∩ (atoms_ty p C)) /\
-    (ε,,A ⊢ l :: B) /\ (ε,,B ⊢ r :: C) /\
-    (r[l .: (↑ >> ids)] ⤳* u) /\ t ⤳* u.
-Proof.
-  intros Ht.
-  pose proof (normalisation _ _ _ Ht) as (u&?&Hnorm).
-  unshelve eapply interpolation_ind in Hnorm as (B&l&r&Hty&Htm&?&?).
-  3: exact (split_s split_emp).
-  unfold interpolate_tm, interpolate_ty in * ; cbn in *.
-  exists B, u, r, l.
-  prod_splitter.
-  - intros p b.
-    specialize (Hty p b) ; cbn in *.
-    intuition.
-  - assumption.
-  - assumption.
-  - etransitivity ; tea.
-    apply ereflexivity.
-    substify ; asimpl ; refold.
-    apply subst_term_morphism ; [|easy].
-    intros [|] ; cbn ; [|easy].
-    renamify ; refold.
-    now rewrite up_id.
-  - assumption. 
-Qed.
