code/theories/Notations.v
@@ -11,10 +11,14 @@ Class HasSemTyping (Ctx Ty Obj : Type) := sem_typing : Ctx -> Ty -> Obj -> Prop.
 Class HasClosedSemTyping (Ty Obj : Type) := cl_sem_typing : Ty -> Obj -> Prop.
 Class HasRed (Obj : Type) := red : relation Obj.
 Class HasORed (Obj : Type) := ored : relation Obj.
+Class HasConv (Ctx Ty Obj : Type) := conv : Ctx -> Ty -> Obj -> Obj -> Prop.
 
 (** The object t has type A in Γ *)
 Notation "Γ '⊢' t '::' T" := (typing Γ T t)
   (at level 101, t at level 59) : typing_scope.
+
+(** The objects t and t' are convertible at type A in Γ *)
+Notation "Γ '⊢' t '≡' t' '::' T" := (conv Γ T t t') (at level 101, t, t' at level 59) : typing_scope.
 
 (** The object t is semantically well-typed in Γ *)
 Notation "Γ '⊩' t '::' T" := (sem_typing Γ T t)
