code/theories/Typing.v
@@ -10,9 +10,14 @@ Import ListNotations.
 Create HintDb typing discriminated. 
 
 Section Typing.
+  Context `{Lang}.
+
   Close Scope typing_scope.
 
   Inductive has_type : context -> type -> term -> Prop :=
+  | _T_Const Γ c :
+    Γ ⊢ (tConst c) :: const_type c
+
   | _T_Var Γ n T :
     in_context n Γ T ->
     Γ ⊢ tVar n :: T
@@ -63,13 +68,13 @@ Section Typing.
 
 End Typing.
 
-#[export] Instance HasTypingTm : HasTyping context type term := has_type.
+#[export] Instance HasTypingTm `{Lang} : HasTyping context type term := has_type.
 
-#[export] Instance HasTypingRen : HasTyping context context ren :=
+#[export] Instance HasTypingRen `{Lang} : HasTyping context context ren :=
   fun (Δ Γ : context) (r : ren) =>
   forall i T, in_context i Γ T -> in_context (r i) Δ T.
 
-#[export] Instance HasTypingSubst : HasTyping context context subst :=
+#[export] Instance HasTypingSubst `{Lang} : HasTyping context context subst :=
  fun (Δ Γ : context) (s : subst) =>
   forall i T, in_context i Γ T -> Δ ⊢ s i :: T.
 
@@ -77,70 +82,79 @@ Ltac fold_typing := change has_type with (typing (Ctx := context) (Ty := type) (
 
 Smpl Add fold_typing : refold.
 
-Lemma T_Var Γ n T :
-    in_context n Γ T ->
-    Γ ⊢ tVar n :: T.
-Proof ltac:(now constructor).
+Section Lemmas.
+  Context `{Lang}.
 
-Lemma T_Star Γ : (Γ ⊢ tStar :: TUnit).
-Proof ltac:(now constructor).
+  Lemma T_Const Γ c :
+      Γ ⊢ tConst c :: const_type c.
+  Proof ltac:(now constructor).
 
-Lemma T_Lam Γ A B t :
-    (Γ ,, A ⊢ t :: B) ->
-    Γ ⊢ tLam t :: TFun A B.
-Proof ltac:(now constructor).
+  Lemma T_Var Γ n T :
+      in_context n Γ T ->
+      Γ ⊢ tVar n :: T.
+  Proof ltac:(now constructor).
 
-Lemma T_App Γ A B f u :
-    (Γ ⊢ f :: TFun A B) ->
-    (Γ ⊢ u :: A) ->
-    Γ ⊢ tApp f u :: B.
-Proof ltac:(now econstructor).
+  Lemma T_Star Γ : (Γ ⊢ tStar :: TUnit).
+  Proof ltac:(now constructor).
 
-Lemma T_Pair Γ A B a b :
-    (Γ ⊢ a :: A) ->
-    (Γ ⊢ b :: B) ->
-    (Γ ⊢ tPair a b :: TProd A B).
-Proof ltac:(now constructor).
+  Lemma T_Lam Γ A B t :
+      (Γ ,, A ⊢ t :: B) ->
+      Γ ⊢ tLam t :: TFun A B.
+  Proof ltac:(now constructor).
 
-Lemma T_Fst Γ A B t :
-    (Γ ⊢ t :: TProd A B) ->
-    (Γ ⊢ tFst t :: A).
-Proof ltac:(now econstructor).
+  Lemma T_App Γ A B f u :
+      (Γ ⊢ f :: TFun A B) ->
+      (Γ ⊢ u :: A) ->
+      Γ ⊢ tApp f u :: B.
+  Proof ltac:(now econstructor).
 
-Lemma T_Snd Γ A B t :
-    (Γ ⊢ t :: TProd A B) ->
-    (Γ ⊢ tSnd t :: B).
-Proof ltac:(now econstructor).
+  Lemma T_Pair Γ A B a b :
+      (Γ ⊢ a :: A) ->
+      (Γ ⊢ b :: B) ->
+      (Γ ⊢ tPair a b :: TProd A B).
+  Proof ltac:(now constructor).
 
-Lemma T_Abort Γ A t :
-    (Γ ⊢ t :: TEmp) ->
-    (Γ ⊢ tAbort t :: A).
-Proof ltac:(now constructor).
+  Lemma T_Fst Γ A B t :
+      (Γ ⊢ t :: TProd A B) ->
+      (Γ ⊢ tFst t :: A).
+  Proof ltac:(now econstructor).
 
-Lemma T_Left Γ A B t :
-    (Γ ⊢ t :: A) ->
-    (Γ ⊢ tLeft t :: TSum A B).
-Proof ltac:(now constructor).
+  Lemma T_Snd Γ A B t :
+      (Γ ⊢ t :: TProd A B) ->
+      (Γ ⊢ tSnd t :: B).
+  Proof ltac:(now econstructor).
 
-Lemma T_Right Γ A B t :
-    (Γ ⊢ t :: B) ->
-    (Γ ⊢ tRight t :: TSum A B).
-Proof ltac:(now constructor).
+  Lemma T_Abort Γ A t :
+      (Γ ⊢ t :: TEmp) ->
+      (Γ ⊢ tAbort t :: A).
+  Proof ltac:(now constructor).
 
-Lemma T_If Γ A B T s bl br :
-    (Γ ⊢ s :: TSum A B) ->
-    (Γ,,A ⊢ bl :: T) ->
-    (Γ,,B ⊢ br :: T) ->
-    (Γ ⊢ tIf s bl br :: T).
-Proof ltac:(now econstructor).
+  Lemma T_Left Γ A B t :
+      (Γ ⊢ t :: A) ->
+      (Γ ⊢ tLeft t :: TSum A B).
+  Proof ltac:(now constructor).
 
-Hint Resolve T_Var T_Star T_Lam T_App T_Pair T_Fst T_Snd T_Abort T_Left T_Right T_If : typing.
+  Lemma T_Right Γ A B t :
+      (Γ ⊢ t :: B) ->
+      (Γ ⊢ tRight t :: TSum A B).
+  Proof ltac:(now constructor).
 
-Lemma var_empty n T : ~ in_context n ε T.
-Proof.
-  unfold in_context ; cbn.
-  discriminate.
-Qed.
+  Lemma T_If Γ A B T s bl br :
+      (Γ ⊢ s :: TSum A B) ->
+      (Γ,,A ⊢ bl :: T) ->
+      (Γ,,B ⊢ br :: T) ->
+      (Γ ⊢ tIf s bl br :: T).
+  Proof ltac:(now econstructor).
+
+  Lemma var_empty n T : ~ in_context n ε T.
+  Proof.
+    unfold in_context ; cbn.
+    discriminate.
+  Qed.
+
+End Lemmas.
+
+Hint Resolve T_Const T_Var T_Star T_Lam T_App T_Pair T_Fst T_Snd T_Abort T_Left T_Right T_If : typing.
 
 Hint Extern 0 (False) => (eapply var_empty) : typing.
 
@@ -148,203 +162,215 @@ Hint Extern 0 (in_context _ _ _) => reflexivity : typing.
 
 (** ** Typing for renamings and substitutions *)
 
-(** Not in the [typing] hint database because it is too wild, needs to be applied directly *)
-Instance ren_has_type_ext (Δ Γ : context) :
-  Proper ((pointwise_relation _ eq) ==> iff) (typing (Obj := ren) Δ Γ).
-Proof.
-  intros ?? Hren. 
-  split ; intros e i T Hin.
-  1: rewrite <- Hren.
-  2: rewrite Hren.
-  all: now apply e.
-Qed.
+Section TypingSubst.
+  Context `{Lang}.
 
-Lemma ren_id_has_type (Δ : context) :
-  Δ ⊢ id :: Δ.
-Proof.
-  now intros i T Hin ; cbn.
-Qed.
+  (** Not in the [typing] hint database because it is too wild, needs to be applied directly *)
+  Instance ren_typing_ext (Δ Γ : context) :
+    Proper ((pointwise_relation _ eq) ==> iff) (typing (Obj := ren) Δ Γ).
+  Proof.
+    intros ?? Hren. 
+    split ; intros e i T Hin.
+    1: rewrite <- Hren.
+    2: rewrite Hren.
+    all: now apply e.
+  Qed.
 
-Lemma ren_comp_has_type (Δ Γ Θ : context) (r r' : ren) :
-  (Δ ⊢ r :: Γ) ->
-  (Γ ⊢ r' :: Θ) ->
-  (Δ ⊢ (r' >> r) :: Θ).
-Proof.
-  intros * Hr Hr' i T Hin.
-  apply Hr', Hr in Hin.
-  assumption.
-Qed.
+  Lemma ren_id_typing (Δ : context) :
+    Δ ⊢ id :: Δ.
+  Proof.
+    now intros i T Hin ; cbn.
+  Qed.
 
-Lemma shift_has_type (Γ : context) (T : type) : (Γ,,T) ⊢ ↑ :: Γ.
-Proof.
-  intros ? ** ; assumption.
-Qed.
-
-Lemma ren_cons_has_type (Δ Γ : context) (T : type) (ρ : ren) (n : nat) :
-  in_context n Δ T ->
-  (Δ ⊢ ρ :: Γ) ->
-  Δ ⊢ (n .: ρ) :: (Γ,,T).
-Proof.
-  intros Hty Hs [] T' Hin ; cbn.
-  - unfold in_context in Hin ; cbn in *.
-    injection Hin ; subst.
+  Lemma ren_comp_typing (Δ Γ Θ : context) (r r' : ren) :
+    (Δ ⊢ r :: Γ) ->
+    (Γ ⊢ r' :: Θ) ->
+    (Δ ⊢ (r' >> r) :: Θ).
+  Proof.
+    intros * Hr Hr' i T Hin.
+    apply Hr', Hr in Hin.
     assumption.
-  - apply Hs, Hin.
-Qed.
+  Qed.
 
-Hint Resolve ren_id_has_type ren_comp_has_type shift_has_type ren_cons_has_type : typing.
+  Lemma shift_typing (Γ : context) (T : type) : (Γ,,T) ⊢ ↑ :: Γ.
+  Proof.
+    intros ? ** ; assumption.
+  Qed.
 
-Lemma ren_lift_has_type (Δ Γ : context) (T : type) (r : ren) :
-  (Δ ⊢ r :: Γ) ->
-  (Δ,,T) ⊢ (⇑ r) ::  (Γ,,T).
-Proof.
-  intros.
-  change (Δ,, T ⊢ 0 .: r >> S :: Γ,, T).
-  eauto with typing.
-Qed.
+  Lemma ren_cons_typing (Δ Γ : context) (T : type) (ρ : ren) (n : nat) :
+    in_context n Δ T ->
+    (Δ ⊢ ρ :: Γ) ->
+    Δ ⊢ (n .: ρ) :: (Γ,,T).
+  Proof.
+    intros Hty Hs [] T' Hin ; cbn.
+    - unfold in_context in Hin ; cbn in *.
+      injection Hin ; subst.
+      assumption.
+    - apply Hs, Hin.
+  Qed.
 
-Hint Resolve ren_lift_has_type : typing.
+  Hint Resolve ren_id_typing ren_comp_typing shift_typing ren_cons_typing : typing.
 
-Lemma ren_typing (Δ Γ : context) (T : type) (t : term) (r : ren) :
-  (Γ ⊢ t :: T) ->
-  (Δ ⊢ r :: Γ) ->
-  Δ ⊢ t⟨r⟩ :: T.
-Proof.
-  intros Ht Hr.
-  induction Ht in Δ, r, Hr ; cbn ; eauto 10 with typing.
-Qed.
+  Lemma ren_up_typing (Δ Γ : context) (T : type) (r : ren) :
+    (Δ ⊢ r :: Γ) ->
+    (Δ,,T) ⊢ (⇑ r) ::  (Γ,,T).
+  Proof.
+    intros.
+    change (Δ,, T ⊢ 0 .: r >> S :: Γ,, T).
+    eauto with typing.
+  Qed.
 
+  Hint Resolve ren_up_typing : typing.
+
+  Lemma ren_typing (Δ Γ : context) (T : type) (t : term) (r : ren) :
+    (Γ ⊢ t :: T) ->
+    (Δ ⊢ r :: Γ) ->
+    Δ ⊢ t⟨r⟩ :: T.
+  Proof.
+    intros Ht Hr.
+    induction Ht in Δ, r, Hr ; cbn ; eauto 10 with typing.
+  Qed.
+
+  Hint Resolve ren_typing : typing.
+
+  (** Same, not in the hint database because it is too wild *)
+  Instance subst_typing_ext (Δ Γ : context) :
+    Proper ((pointwise_relation _ eq) ==> iff) (typing (Obj := subst) Δ Γ).
+  Proof.
+    intros ?? Hsubst.
+    split ; intros e i T Hin.
+    1: rewrite <- Hsubst.
+    2: rewrite Hsubst.
+    all: now apply e.
+  Qed.
+
+  Lemma typing_emp `{Lang} Γ (σ : subst) : Γ ⊢ σ :: ε.
+  Proof.
+    intros ? **.
+    exfalso.
+    eauto with typing.
+  Qed.
+
+  Lemma ren_subst_typing (Δ Γ Θ : context) (r : ren) (σ : subst) :
+    (Δ ⊢ σ :: Γ) ->
+    (Γ ⊢ r :: Θ) ->
+    (Δ ⊢ (r >> σ) :: Θ).
+  Proof.
+    intros Hs Hr i T Hin ; cbn.
+    now apply Hs, Hr.
+  Qed.
+
+  Lemma subst_ren_typing (Δ Γ Θ : context) (r : ren) (σ : subst) :
+    (Δ ⊢ r :: Γ) ->
+    (Γ ⊢ σ :: Θ) ->
+    (Δ ⊢ (σ >> ren1 r) :: Θ).
+  Proof.
+    intros Hs Hr i T Hin ; cbn.
+    eauto with typing.
+  Qed.
+
+  Lemma subst_cons_typing (Δ Γ : context) (T : type) (σ : subst) (t : term) :
+    (Δ ⊢ t :: T) ->
+    (Δ ⊢ σ :: Γ) ->
+    Δ ⊢ (t .: σ) :: (Γ,,T).
+  Proof.
+    intros Hty Hs [] T' Hin ; cbn.
+    - unfold in_context in Hin ; cbn in *.
+      injection Hin ; subst.
+      assumption.
+    - apply Hs, Hin.
+  Qed.
+
+  Hint Resolve ren_subst_typing subst_ren_typing subst_cons_typing : typing.
+
+  Lemma id_subst_typing (Γ : context) :
+    Γ ⊢ ids :: Γ.
+  Proof.
+    intros ?? ? ; cbn.
+    eauto with typing.
+  Qed.
+
+  Hint Resolve id_subst_typing : typing.
+
+  Lemma subst_one_typing (Γ : context) (T : type) (t : term) :
+    (Γ ⊢ t :: T) -> 
+    Γ ⊢ (t..) ::  (Γ,,T).
+  Proof.
+    eauto with typing.
+  Qed.
+
+  Lemma subst_lift_typing (Δ Γ : context) (T : type) (σ : subst) :
+    (Δ ⊢ σ :: Γ) ->
+    (Δ,,T) ⊢ (⇑ σ) :: (Γ,,T).
+  Proof.
+    intros.
+    eapply subst_cons_typing.
+    all: eauto with typing.
+  Qed.
+
+  Hint Resolve subst_one_typing subst_lift_typing : typing.
+
+  Lemma subst_typing (Δ Γ : context) t T (σ : subst) :
+    (Γ ⊢ t :: T) ->
+    (Δ ⊢ σ :: Γ) ->
+    Δ ⊢ t[σ] :: T.
+  Proof.
+    intros Ht Hσ.
+    induction Ht in Δ, σ, Hσ ; cbn ; eauto 10 with typing.
+  Qed.
+
+  Hint Resolve subst_typing : typing.
+
+  Lemma subst_comp_typing (Δ Γ Θ : context) (σ σ' : subst) :
+    (Δ ⊢ σ :: Γ) ->
+    (Γ ⊢ σ' :: Θ) ->
+    (Δ ⊢ (σ' >> (subst_term σ)) :: Θ).
+  Proof.
+    do 2 red.
+    eauto with typing.
+  Qed.
+
+  Lemma tip_typing (Γ : context) (A B : type) (f : term -> term) :
+    (Γ,,A ⊢ f (tVar 0) :: B) ->
+    (Γ,,A ⊢ tip f :: Γ,,B).
+  Proof.
+    unfold tip.
+    eauto with typing.
+  Qed.
+
+  Lemma swap_var_typing Γ (A B : type) :
+    ((Γ,,A),,B) ⊢ swap_var :: ((Γ,,B),,A).
+  Proof.
+    unfold swap_var.
+    eauto with typing.
+  Qed.
+
+End TypingSubst.
+
+Hint Immediate typing_emp : typing.
+Hint Resolve ren_id_typing ren_comp_typing shift_typing ren_cons_typing : typing.
+Hint Resolve ren_up_typing : typing.
 Hint Resolve ren_typing : typing.
-
-(** Same, not in the hint database because it is too wild *)
-Instance subst_has_type_ext (Δ Γ : context) :
-  Proper ((pointwise_relation _ eq) ==> iff) (typing (Obj := subst) Δ Γ).
-Proof.
-  intros ?? Hsubst.
-  split ; intros e i T Hin.
-  1: rewrite <- Hsubst.
-  2: rewrite Hsubst.
-  all: now apply e.
-Qed.
-
-Lemma ren_subst_has_type (Δ Γ : context) (r : ren) :
-  (Δ ⊢ r :: Γ) ->
-  (Δ ⊢ (r >> ids) :: Γ).
-Proof.
-  intros Hr i T Hin ; cbn.
-  constructor.
-  now apply Hr.
-Qed.
-
-Lemma subst_cons_has_type (Δ Γ : context) (T : type) (σ : subst) (t : term) :
-  (Δ ⊢ t :: T) ->
-  (Δ ⊢ σ :: Γ) ->
-  Δ ⊢ (t .: σ) :: (Γ,,T).
-Proof.
-  intros Hty Hs [] T' Hin ; cbn.
-  - unfold in_context in Hin ; cbn in *.
-    injection Hin ; subst.
-    assumption.
-  - apply Hs, Hin.
-Qed.
-
-Hint Resolve ren_subst_has_type subst_cons_has_type : typing.
-
-Lemma id_subst_has_type (Γ : context) :
-  Γ ⊢ ids :: Γ.
-Proof.
-  eauto with typing.
-Qed.
-
-Lemma subst_one_has_type (Γ : context) (T : type) (t : term) :
-  (Γ ⊢ t :: T) -> 
-  Γ ⊢ (t..) ::  (Γ,,T).
-Proof.
-  intros.
-  eauto with typing.
-Qed.
-
-Lemma subst_lift_has_type (Δ Γ : context) (T : type) (σ : subst) :
-  (Δ ⊢ σ :: Γ) ->
-  (Δ,,T) ⊢ (⇑ σ) :: (Γ,,T).
-Proof.
-  intros.
-  eapply subst_cons_has_type.
-  1: eauto with typing.
-  do 2 red ; cbn.
-  eauto with typing.
-Qed.
-
-Hint Resolve id_subst_has_type subst_one_has_type subst_lift_has_type : typing.
-
-Lemma subst_typing (Δ Γ : context) t T (σ : subst) :
-  (Γ ⊢ t :: T) ->
-  (Δ ⊢ σ :: Γ) ->
-  Δ ⊢ t[σ] :: T.
-Proof.
-  intros Ht Hσ.
-  induction Ht in Δ, σ, Hσ ; cbn ; eauto 10 with typing.
-Qed.
-
+Hint Resolve ren_subst_typing subst_ren_typing subst_cons_typing : typing.
+Hint Resolve id_subst_typing subst_one_typing subst_lift_typing : typing.
 Hint Resolve subst_typing : typing.
+Hint Resolve subst_comp_typing tip_typing swap_var_typing : typing.
 
-Lemma subst_comp_has_type (Δ Γ Θ : context) (σ σ' : subst) :
-  (Δ ⊢ σ :: Γ) ->
-  (Γ ⊢ σ' :: Θ) ->
-  (Δ ⊢ (σ' >> (subst_term σ)) :: Θ).
+
+Lemma term_up_eq `{Lang} (Γ : context) (A : type) (σ σ' : subst) :
+  (forall i T, in_context i Γ T -> σ i = σ' i) ->
+  forall i T, in_context i (Γ,,A) T -> (⇑ σ) i = (⇑ σ') i.
 Proof.
-  do 2 red.
-  eauto with typing.
+  intros e [|] ? ? ; cbn.
+  1: easy.
+  now erewrite e.
 Qed.
 
-Lemma tip_has_type (Γ : context) (A B : type) (f : term -> term) :
-  (Γ,,A ⊢ f (tVar 0) :: B) ->
-  (Γ,,A ⊢ tip f :: Γ,,B).
+Lemma term_ext_closed `{Lang} (Γ : context) (A : type) (t : term) (σ σ' : subst) :
+  (Γ ⊢ t :: A) ->
+  (forall i T, in_context i Γ T -> σ i = σ' i) ->
+  t[σ] = t[σ'].
 Proof.
-  unfold tip.
-  eauto with typing.
-Qed.
-
-Lemma swap_var_has_type Γ (A B : type) :
-  ((Γ,,A),,B) ⊢ swap_var :: ((Γ,,B),,A).
-Proof.
-  unfold swap_var.
-  eauto with typing.
-Qed.
-
-Hint Resolve subst_comp_has_type tip_has_type swap_var_has_type : typing.
-
-(** ** Types have decidable equality *)
-
-Fixpoint eqb_ty (T T' : type) : bool :=
-  match T, T' with
-  | TBase b, TBase b' => eqb_base b b'
-  | TUnit, TUnit | TEmp, TEmp => true
-  | TFun A B, TFun A' B' | TProd A B, TProd A' B' | TSum A B, TSum A' B' =>
-    eqb_ty A A' && eqb_ty B B'
-  | _, _ => false
-  end.
-
-Lemma eqb_ty_refl T : eqb_ty T T = true.
-Proof.
-  induction T ; cbn ; eauto.
-  1: apply eqb_base_refl.
-  all: rewrite IHT1 ; cbn ; assumption.
-Qed.
-
-Lemma eqb_ty_sound T T' : eqb_ty T T' = true -> T = T'.
-Proof.
-  induction T in T' |- * ; destruct T' ; cbn ; try solve [easy|congruence].
-  1: now intros ->%eqb_base_sound.
-  all: intros []%andb_prop ; now f_equal.
-Qed.
-
-Lemma eqb_ty_correct T T' : reflect (T = T') (eqb_ty T T').
-Proof.
-  destruct (eqb_ty T T') eqn:e.
-  all: constructor.
-  - now apply eqb_ty_sound.
-  - intros ? ; subst.
-    rewrite eqb_ty_refl in e.
-    congruence.
+  intros Hty Hin.
+  induction Hty in σ, σ', Hin |- * ; cbn ; refold ; f_equal ; eauto using term_up_eq.
 Qed.
