code/theories/Languages.v
@@ -1,0 +1,169 @@
+From Stdlib Require Import Relations Arith Lia Bool List RelationClasses.
+From stdpp Require Import propset.
+From Interpolation Require Import Utils Syntax.
+
+(** ** Atoms of a type/context *)
+
+Section AtomsTy.
+  Context `{Ba : Base}.
+
+  Fixpoint atoms_ty (p : polarity) (A : type) {struct A} : propset base :=
+    match A with
+    | TBase b => if p then {[b]} else ∅
+    | TUnit | TEmp => ∅
+    | TFun A B => atoms_ty (negp p) A ∪ atoms_ty p B
+    | TProd A B | TSum A B => atoms_ty p A ∪ atoms_ty p B
+    end.
+
+  Fixpoint atoms_ctx (p : polarity) (Γ : context) : propset base :=
+    match Γ with
+    | nil => ∅
+    | cons A Γ => atoms_ctx p Γ ∪ (atoms_ty p A)
+    end.
+
+  Lemma atoms_in n Γ T :
+    in_context n Γ T ->
+    (forall p, atoms_ty p T ⊆ atoms_ctx p Γ).
+  Proof.
+    intros H.
+    unfold in_context in *.
+    induction n in Γ, H |- * ; cbn.
+    - destruct Γ ; cbn in * ; [congruence|].
+      intros ? ? ?.
+      set_solver.
+    - destruct Γ ; cbn in * ; [congruence|].
+      intros ?.
+      set_solver.
+  Qed.
+
+End AtomsTy.
+
+Section AtomsTm.
+  Context `{Lang}.
+
+  Definition atoms_const (p : polarity) (P : propset const) : propset base :=
+    {[ b | exists c, (c ∈ P) /\ b ∈ atoms_ty p (const_type c) ]}.
+
+  Record const_split :=
+  {
+    pconst_l : propset const ;
+    pconst_r : propset const ;
+    const_cover : forall c, (c ∈ pconst_l) + (c ∈ pconst_r) 
+  }.
+
+  Definition flip_csplit (s : const_split) := {|
+    pconst_l := s.(pconst_r) ;
+    pconst_r := s.(pconst_l) ;
+    const_cover := (fun c => match (s.(const_cover) c) with | inl p => inr p | inr p => inl p end)
+  |}.
+
+  Fixpoint atoms_tm (t : term) {struct t} : propset const :=
+    match t with
+    | tConst c => {[c]}
+    | tVar _ | tStar => ∅
+    | tProj _ t | tLam t | tAbort t | tIn _ t => atoms_tm t
+    | tPair t t' | tApp t t' => atoms_tm t ∪ atoms_tm t'
+    | tIf s bl br => atoms_tm s ∪ atoms_tm bl ∪ atoms_tm br
+    end.
+
+  Lemma atoms_ren t ρ : atoms_tm (t⟨ρ⟩) ≡ atoms_tm t.
+  Proof.
+    set_unfold.
+    intros c.
+    induction t in ρ |- * ; cbn ; set_solver.
+  Qed.
+
+  Definition atoms_subst (σ : subst) : propset const :=
+    {[ c | exists i, c ∈ atoms_tm (σ i) ]}.
+
+  Instance atoms_subst_ext : Proper (pointwise_relation _ (=) ==> (≡)) atoms_subst.
+  Proof.
+    intros ?? e.
+    unfold atoms_subst.
+    set_unfold.
+    intros c.
+    now setoid_rewrite e.
+  Qed.
+
+  Lemma atoms_subst_ren ρ : atoms_subst (ρ >> ids) ≡ ∅.
+  Proof.
+    set_unfold.
+    intros ? [] ; now cbn in *.
+  Qed.
+    
+  Corollary atoms_subst_id : atoms_subst ids ≡ ∅.
+  Proof.
+    set_unfold.
+    intros ? [] ; now cbn in *.
+  Qed.
+
+  Lemma atoms_subst_cons t σ : atoms_subst (t .: σ) ≡ (atoms_tm t) ∪ (atoms_subst σ).
+  Proof.
+    set_unfold.
+    intros c.
+    split.
+    - intros [[|] ] ; cbn in * ; cbn.
+      all: set_solver.
+    - intros [|[]].
+      1: exists 0.
+      2: eexists (S _).
+      all: cbn; set_solver.
+  Qed.
+
+  Corollary atoms_subst_tip f : atoms_subst (tip f) ≡ atoms_tm (f (tVar 0)).
+  Proof.
+    unfold tip.
+    rewrite atoms_subst_cons, atoms_subst_ren.
+    set_solver.
+  Qed.
+
+  Corollary atoms_subst_up (σ : subst) : atoms_subst (⇑ σ) ≡ atoms_subst σ.
+  Proof.
+    set_unfold.
+    intros c.
+    split.
+    - intros [[|] Hin] ; cbn in * ; refold.
+      1: exfalso ; now set_solver.
+      eexists.
+      now rewrite atoms_ren in Hin.
+    - intros [].
+      eexists (S _) ; cbn ; refold.
+      now rewrite atoms_ren.
+  Qed.
+
+  Lemma atoms_tm_subst (t : term) (σ : subst) :
+    atoms_tm (t[σ]) ⊆ atoms_tm t ∪ atoms_subst σ.
+  Proof.
+    induction t in σ |- * ; cbn.
+    - unfold atoms_subst.
+      set_unfold.
+      intros.
+      right.
+      now eexists.
+    - set_solver.
+    - set_solver.
+    - specialize (IHt1 σ).
+      specialize (IHt2 σ).
+      set_solver.
+    - specialize (IHt σ).
+      set_solver.
+    - refold.
+      specialize (IHt (⇑ σ)).
+      rewrite atoms_subst_up in IHt.
+      set_solver.
+    - specialize (IHt1 σ).
+      specialize (IHt2 σ).
+      set_solver.
+    - specialize (IHt σ).
+      set_solver.
+    - specialize (IHt σ).
+      set_solver.
+    - refold.
+      specialize (IHt1 σ).
+      specialize (IHt2 (⇑ σ)).
+      specialize (IHt3 (⇑ σ)).
+      rewrite atoms_subst_up in IHt2, IHt3.
+      set_solver.
+  Qed.
+
+End AtomsTm.
