code/theories/MetaTheory.v
@@ -3,685 +3,722 @@ From Stdlib Require Import Relations Arith Lia Bool List.
 
 (** ** Preservation of typing under reduction *)
 
-Lemma preservation_one (Γ : context) (T : type) (t u : term) : (Γ ⊢ t :: T) -> t ⤳ u -> (Γ ⊢ u :: T).
-Proof.
-  intros Hty Hred.
-  induction Hred in Γ, T, Hty |- *.
-  all: try (match goal with | e : elim |- _ => destruct e ; cbn in * end ; try solve [congruence]).
-  all: try (match goal with | e : _ = _ |- _ => inversion e ; subst end).
-  all: repeat match goal with | H : (_ ⊢ _ _ :: _) |- _ => inversion H ; subst ; clear H ; refold end.
-  all: eauto 20 with typing.
-Qed.
+Section Safety.
+  Context `{Lang}.
 
-Lemma preservation (Γ : context) (T : type) (t u : term) : (Γ ⊢ t :: T) -> t ⤳* u -> (Γ ⊢ u :: T).
-Proof.
-  induction 2 ; eauto using preservation_one.
-Qed.
+  Lemma preservation_one (Γ : context) (T : type) (t u : term) : (Γ ⊢ t :: T) -> t ⤳ u -> (Γ ⊢ u :: T).
+  Proof.
+    intros Hty Hred.
+    induction Hred in Γ, T, Hty |- *.
+    all: try (match goal with | e : elim |- _ => destruct e ; cbn in * end ; try solve [congruence]).
+    all: try (match goal with | e : _ = _ |- _ => inversion e ; subst end).
+    all: repeat match goal with | H : (_ ⊢ _ _ :: _) |- _ => inversion H ; subst ; clear H ; refold end.
+    all: eauto 20 with typing.
+  Qed.
 
-(** ** Progress *)
-(** A well-typed term is either a normal form, or can do a reduction step*)
+  Lemma preservation (Γ : context) (T : type) (t u : term) : (Γ ⊢ t :: T) -> t ⤳* u -> (Γ ⊢ u :: T).
+  Proof.
+    induction 2 ; eauto using preservation_one.
+  Qed.
 
-Lemma progress (Γ : context) (T : type) (t : term) :
-  (Γ ⊢ t :: T) -> (Γ ⊢ t ◃ T) \/ (exists u, t ⤳ u).
-Proof.
-  intros Hty.
-  induction Hty ; refold.
-  all: repeat match goal with
-    | IH : _ \/ _ |- _ => destruct IH as [?|[]] ; [|right ; eexists ; now econstructor] end.
-  all: try solve [left ; eauto with typing].
-  all: match goal with
-      | IH : _ ⊢ _ ◃ (_ _) |- _ => (inversion IH ; subst ; clear IH)
-      | IH : _ ⊢ _ ◃ TEmp |- _ => inversion IH ; subst ; clear IH
-    end ;
-    try solve [right ; eexists ; now constructor].
-  all: left ; eauto with typing.
-Qed.
+  (** ** Progress *)
+  (** A well-typed term is either a normal form, or can do a reduction step*)
 
-(** ** Bidirectional typing characterises well-typed normal forms *)
+  Lemma progress (Γ : context) (T : type) (t : term) :
+    (Γ ⊢ t :: T) -> (Γ ⊢ t ◃ T) \/ (exists u, t ⤳ u).
+  Proof.
+    intros Hty.
+    induction Hty ; refold.
+    all: repeat match goal with
+      | IH : _ \/ _ |- _ => destruct IH as [?|[]] ; [|right ; eexists ; now econstructor] end.
+    all: try solve [left ; eauto with typing].
+    all: match goal with
+        | IH : _ ⊢ _ ◃ (_ _) |- _ => (inversion IH ; subst ; clear IH)
+        | IH : _ ⊢ _ ◃ TEmp |- _ => inversion IH ; subst ; clear IH
+      end ;
+      try solve [right ; eexists ; now constructor].
+    all: left ; eauto with typing.
+  Qed.
 
-Lemma bidir_normal_ind : bidir_concl
-  (fun Γ T t => forall u, t ⤳ u -> False)
-  (fun Γ T t => forall u, t ⤳ u -> False).
-Proof.
-  apply bidir_ind ; intros ; eauto.
-  all: match goal with H : _ ⤳ _ |- _ => inversion H ; subst ; refold ; clear H end ; eauto.
-  all: match goal with H : _ ⊢ _ ▹ _ |- _ => inversion H end.
-Qed.
+  (** ** Bidirectional typing characterises well-typed normal forms *)
 
-Lemma normal_bidir Γ T t :
-  (Γ ⊢ t ◃ T) <-> ((Γ ⊢ t :: T) /\ ~(exists u, t ⤳ u)).
-Proof.
-  split.
-  - intros Hty.
+  Lemma bidir_normal_ind : bidir_concl
+    (fun Γ T t => forall u, t ⤳ u -> False)
+    (fun Γ T t => forall u, t ⤳ u -> False).
+  Proof.
+    apply bidir_ind ; intros ; eauto.
+    all: match goal with H : _ ⤳ _ |- _ => inversion H ; subst ; refold ; clear H end ; eauto.
+    all: match goal with H : _ ⊢ _ ▹ _ |- _ => inversion H end.
+  Qed.
+
+  Lemma normal_bidir Γ T t :
+    (Γ ⊢ t ◃ T) <-> ((Γ ⊢ t :: T) /\ ~(exists u, t ⤳ u)).
+  Proof.
     split.
-    + now apply bidir_typing in Hty.
-    + intros [? Hu].
-      now eapply bidir_normal_ind in Hty.
-  - intros [Hty ].
-    now apply progress in Hty as [|].
-Qed.
+    - intros Hty.
+      split.
+      + now apply bidir_typing in Hty.
+      + intros [? Hu].
+        now eapply bidir_normal_ind in Hty.
+    - intros [Hty ].
+      now apply progress in Hty as [|].
+  Qed.
 
+  Lemma nf_red_eq Γ T t t' :
+    (Γ ⊢ t ◃ T) ->
+    t ⤳* t' ->
+    t = t'.
+  Proof.
+    intros Hnf Hred.
+    revert Hnf.
+    pattern t.
+    revert t Hred.
+    apply clos_refl_trans_ind_right.
+    1: easy.
+    intros.
+    exfalso.
+    eapply normal_bidir ; tea.
+    now eexists.
+  Qed.
 
-
+End Safety.
 
 
 (** ** Normalisation *)
 
-(** *** Covering *)
-(** A term is covered by a predicate if it is a case tree, with nodes eliminations of
-  neutrals of sum and empty types, and leaves terms that satisfy the predicate. *)
-Inductive covered (F : context -> term -> Prop) (Γ : context) : term -> Prop :=
-| cover_abort t : (Γ ⊢ t ▹ TEmp) -> covered F Γ (tAbort t)
-| cover_if A B s bl br :
-    (Γ ⊢ s ▹ TSum A B) ->
-    covered F (Γ,,A) bl -> covered F (Γ,,B) br ->
-    covered F Γ (tIf s bl br)
-| cover_ret t : F Γ t -> covered F Γ t.
+Section Normalisation.
+  Context `{Lang}.
 
-(** This forms a monad *)
-Definition map_cover F G Γ t : (forall Δ t, F Δ t -> G Δ t) -> covered F Γ t -> covered G Γ t.
-Proof.
-  intros f.
-  induction 1 ; now econstructor.
-Qed.
+  (** *** Covering *)
+  (** A term is covered by a predicate if it is a case tree, with nodes eliminations of
+    neutrals of sum and empty types, and leaves terms that satisfy the predicate. *)
+  Inductive covered (F : context -> term -> Prop) (Γ : context) : term -> Prop :=
+  | cover_abort t : (Γ ⊢ t ▹ TEmp) -> covered F Γ (tAbort t)
+  | cover_if A B s bl br :
+      (Γ ⊢ s ▹ TSum A B) ->
+      covered F (Γ,,A) bl -> covered F (Γ,,B) br ->
+      covered F Γ (tIf s bl br)
+  | cover_ret t : F Γ t -> covered F Γ t.
 
-Definition join_cover F Γ t : covered (covered F) Γ t -> covered F Γ t.
-Proof.
-  induction 1.
-  3: assumption.
-  all: now econstructor.
-Qed.
+  (** This forms a monad *)
+  Definition map_cover F G Γ t : (forall Δ t, F Δ t -> G Δ t) -> covered F Γ t -> covered G Γ t.
+  Proof.
+    intros f.
+    induction 1 ; now econstructor.
+  Qed.
 
-(** And can be run on normal forms to yield a normal form *)
-Definition covered_nf Γ T t : covered (fun Δ t => Δ ⊢ t ◃ T) Γ t -> Γ ⊢ t ◃ T.
-Proof.
-  induction 1 ; eauto with typing.
-Qed.
+  Definition join_cover F Γ t : covered (covered F) Γ t -> covered F Γ t.
+  Proof.
+    induction 1.
+    3: assumption.
+    all: now econstructor.
+  Qed.
 
-(** *** Reducibility *)
+  (** And can be run on normal forms to yield a normal form *)
+  Definition covered_nf Γ T t : covered (fun Δ t => Δ ⊢ t ◃ T) Γ t -> Γ ⊢ t ◃ T.
+  Proof.
+    induction 1 ; eauto with typing.
+  Qed.
 
-(** A term is reducible if it reduces to a value *)
-Definition _reducible (c : context -> type -> term -> Prop) (Γ : context) (T : type) (t : term) :=
-  exists t', t ⤳* t' /\ c Γ T t'.
+  (** *** Reducibility *)
 
-(**
-  A value at positive type is a cover of "proper values", which are either neutrals or constructors.
-  A value at negative type is a normal form that, when observed, yields reducible terms. *)
+  (** A term is reducible if it reduces to a value *)
+  Definition _reducible (c : context -> type -> term -> Prop) (Γ : context) (T : type) (t : term) :=
+    exists t', t ⤳* t' /\ c Γ T t'.
 
-Fixpoint value (Γ : context) (T : type) (t : term) : Prop :=
-  match T with
-  | TBase _ | TEmp => covered (fun Δ u => Δ ⊢ u ▹ T) Γ t
-  | TUnit => (Γ ⊢ t ◃ T)
-  | TSum A B => covered
-    (fun Δ u => (Δ ⊢ u ▹ T) \/
-      (exists a, u = tLeft a /\ value Δ A a) \/ (exists b, u = tRight b /\ value Δ B b))
-    Γ t
-  | TProd A B => (Γ ⊢ t ◃ T) /\ (forall (b : bool), _reducible value Γ (if b then A else B) (tProj b t))
-  | TFun A B => (Γ ⊢ t ◃ T) /\
-      (forall Δ u ρ, (Δ ⊢ ρ :: Γ) -> value Δ A u ->
-        _reducible value Δ B (tApp t⟨ρ⟩ u))
-  end.
+  (**
+    A value at positive type is a cover of "proper values", which are either neutrals or constructors.
+    A value at negative type is a normal form that, when observed, yields reducible terms. *)
 
-Notation reducible := (_reducible value).
+  Fixpoint value (Γ : context) (T : type) (t : term) : Prop :=
+    match T with
+    | TBase _ | TEmp => covered (fun Δ u => Δ ⊢ u ▹ T) Γ t
+    | TUnit => (Γ ⊢ t ◃ T)
+    | TSum A B => covered
+      (fun Δ u => (Δ ⊢ u ▹ T) \/
+        (exists a, u = tLeft a /\ value Δ A a) \/ (exists b, u = tRight b /\ value Δ B b))
+      Γ t
+    | TProd A B => (Γ ⊢ t ◃ T) /\ (forall (b : bool), _reducible value Γ (if b then A else B) (tProj b t))
+    | TFun A B => (Γ ⊢ t ◃ T) /\
+        (forall Δ u ρ, (Δ ⊢ ρ :: Γ) -> value Δ A u ->
+          _reducible value Δ B (tApp t⟨ρ⟩ u))
+    end.
 
-(** *** Semantic typing *)
+  Notation reducible := (_reducible value).
 
-(** A reducible environment is one where all values are reducible *)
-Definition reducible_env (Δ Γ : context) (γ : subst) : Prop :=
-  forall i T, in_context i Γ T -> value Δ T (γ i).
+  (** *** Semantic typing *)
 
-Instance sem_typing_env : HasSemTyping context context subst := reducible_env.
+  (** A reducible environment is one where all values are reducible *)
+  Definition reducible_env (Δ Γ : context) (γ : subst) : Prop :=
+    forall i T, in_context i Γ T -> value Δ T (γ i).
 
-(** A term is semantically well-typed if it yields reducible values in any reducible environment *)
-Definition sem_has_type (Γ : context) (T : type) (t : term) : Prop :=
-  forall (Δ : context) (γ : subst), (Δ ⊩ γ :: Γ) -> reducible Δ T t[γ].
+  Instance sem_has_type_env : HasSemTyping context context subst := reducible_env.
 
-Instance sem_typing_term : HasSemTyping context type term := sem_has_type.
+  (** A term is semantically well-typed if it yields reducible values in any reducible environment *)
+  Definition sem_has_type (Γ : context) (T : type) (t : term) : Prop :=
+    forall (Δ : context) (γ : subst), (Δ ⊩ γ :: Γ) -> reducible Δ T t[γ].
 
-Ltac fold_sem_typing :=
-  change sem_has_type with
-    (sem_typing (Ctx := context) (Ty := type) (Obj := term)) in * ;
-  change reducible_env with
-    (sem_typing (Ctx := context) (Ty := context) (Obj := subst)) in *.
+  Instance sem_has_type_term : HasSemTyping context type term := sem_has_type.
 
-Smpl Add fold_sem_typing : refold.
+  Ltac fold_sem_has_type :=
+    change sem_has_type with
+      (sem_typing (Ctx := context) (Ty := type) (Obj := term)) in * ;
+    change reducible_env with
+      (sem_typing (Ctx := context) (Ty := context) (Obj := subst)) in *.
 
-(** *** Easy lemmas on reducibility *)
-Lemma value_red Γ T t : value Γ T t -> reducible Γ T t.
-Proof.
-  intros.
-  eexists ; split ; eauto ; reflexivity.
-Qed. 
+  Smpl Add fold_sem_has_type : refold.
 
-Lemma red_antired {Γ T t} t' : reducible Γ T t' -> t ⤳* t' -> reducible Γ T t.
-Proof.
-  intros [v] ?.
-  exists v.
-  split ; [|easy].
-  now etransitivity.
-Qed.
-
-(** *** Reify/reflect *)
-(** Neutrals are always values, and values are always normal forms. *)
-
-Hint Extern 0 => (progress subst) : typing.
-
-Lemma reify (T : type) (Γ : context) (t : term) : value Γ T t -> Γ ⊢ t ◃ T.
-Proof.
-  induction T in Γ, t |- * ; cbn ; refold ; try easy.
-  all: intros ; eapply covered_nf, map_cover ; tea.
-  all: cbn ; eauto with typing.
-  intros * [|[[]|[]]].
-  all: cbn ; intuition eauto with typing.
-Qed.
-
-Lemma reflect (T : type) :
-  (forall Γ t, (Γ ⊢ t ▹ T) -> value Γ T t).
-Proof.
-  induction T ; cbn ; refold.
-  all: try solve [now econstructor].
-  - intros * Hne.
-    split ; [eauto with typing|].
-    intros b.
-    apply value_red.
-    assert (Γ ⊢ tProj b t ▹ (if b then T1 else T2)) by now econstructor.
-    destruct b ; solve [now apply IHT1|now apply IHT2].
-  - intros.
-    split.
-    1: now eauto with typing.
+  (** *** Easy lemmas on reducibility *)
+  Lemma value_red Γ T t : value Γ T t -> reducible Γ T t.
+  Proof.
     intros.
-    eapply value_red, IHT2.
-    econstructor.
-    1: now eauto with typing.
-    now apply reify.
-Qed.
+    eexists ; split ; eauto ; reflexivity.
+  Qed. 
 
-(** *** Reducibility is stable under weakening *)
-
-Lemma ren_covered (F : context -> term -> Prop) (Δ Γ : context) (t : term) (r : ren) :
-  (forall Δ Γ ρ t, F Γ t -> (Δ ⊢ ρ :: Γ) -> F Δ t⟨ρ⟩) ->
-  (Δ ⊢ r :: Γ) ->
-  covered F Γ t ->
-  covered F Δ t⟨r⟩.
-Proof.
-  intros HF Hren Hcov.
-  induction Hcov in Δ, r, Hren |- * ; cbn ; econstructor ; now eauto with typing.
-Qed.
-
-Lemma ren_value (Δ Γ : context) (T : type) (t : term) (r : ren) :
-  value Γ T t ->
-  (Δ ⊢ r :: Γ) ->
-  value Δ T t⟨r⟩.
-Proof.
-  intros Hval Hren.
-  induction T in Γ, Δ, t, r, Hren, Hval |- * ; cbn in *;
-    try solve [intuition eauto using ren_covered with typing].
-  - split ; [intuition eauto with typing|].
-    intros b.
-    destruct Hval as [_ Hval].
-    specialize (Hval b) as [u Hu].
-    exists (u⟨r⟩).
-    split ; [|now destruct b ; intuition eauto with typing].
-    change (tProj b t⟨r⟩) with ((tProj b t)⟨r⟩).
-    now apply R_ren.
-  - split ; [intuition eauto with typing|].
-    intros Ξ **.
-    edestruct Hval as [_ [v ]].
-    1: eapply ren_comp_has_type ; cycle -1 ; eassumption.
-    1: eassumption.
+  Lemma red_antired {Γ T t} t' : reducible Γ T t' -> t ⤳* t' -> reducible Γ T t.
+  Proof.
+    intros [v] ?.
     exists v.
-    now asimpl ; refold.
-  - eapply ren_covered ; tea.
-    intros ?? r' ? Hval' **.
-    destruct Hval' as [|[[a [->]]|[b [->]]]].
-    + left ; eauto with typing.
-    + right ; left.
-      now exists (a⟨r'⟩).
-    + right ; right.
-      now exists b⟨r'⟩.
-Qed.
+    split ; [|easy].
+    now etransitivity.
+  Qed.
 
-Lemma sem_ren_subst (Ξ Δ Γ : context) (γ : subst) (r : ren) :
-  (Δ ⊩ γ :: Γ) ->
-  (Ξ ⊢ r :: Δ) ->
-  Ξ ⊩ γ >> ren_term r :: Γ.
-Proof.
-  intros Hγ ? i **.
-  cbn.
-  now eapply ren_value.
-Qed.
+  (** *** Reify/reflect *)
+  (** Neutrals are always values, and values are always normal forms. *)
 
-(** *** Semantic typing of various substitutions *)
+  Hint Extern 0 => (progress subst) : typing.
 
-Lemma sem_Up {Δ Γ : context} {A : type} {γ : subst} : (Δ ⊩ γ :: Γ) -> (Δ,,A) ⊩ ⇑ γ :: (Γ ,, A).
-Proof.
-  intros Hγ [|] T ? ; cbn in * ; refold.
-  - apply reflect ; eauto with typing.
-  - eapply ren_value ; eauto with typing.
-Qed.
+  Lemma reify (T : type) (Γ : context) (t : term) : value Γ T t -> Γ ⊢ t ◃ T.
+  Proof.
+    induction T in Γ, t |- * ; cbn ; refold ; try easy.
+    all: intros ; eapply covered_nf, map_cover ; tea.
+    all: cbn ; eauto with typing.
+    intros * [|[[]|[]]].
+    all: cbn ; intuition eauto with typing.
+  Qed.
 
-Lemma sem_cons (Δ Γ : context) (A : type) (γ : subst) (t : term) :
-  (Δ ⊩ γ :: Γ) ->
-  value Δ A t ->
-  Δ ⊩ t .: γ :: (Γ ,, A).
-Proof.
-  intros Hγ Ht [|] ? Hin ; cbn.
-  - now inversion Hin ; subst.
-  - now apply Hγ.
-Qed.
+  Lemma reflect (T : type) :
+    (forall Γ t, (Γ ⊢ t ▹ T) -> value Γ T t).
+  Proof.
+    induction T ; cbn ; refold.
+    all: try solve [now econstructor].
+    - intros * Hne.
+      split ; [eauto with typing|].
+      intros b.
+      apply value_red.
+      assert (Γ ⊢ tProj b t ▹ (if b then T1 else T2)) by now econstructor.
+      destruct b ; solve [now apply IHT1|now apply IHT2].
+    - intros.
+      split.
+      1: now eauto with typing.
+      intros.
+      eapply value_red, IHT2.
+      econstructor.
+      1: now eauto with typing.
+      now apply reify.
+  Qed.
 
-(** *** We can push eliminators to the leaves of a cover *)
+  (** *** Reducibility is stable under weakening *)
 
-Lemma proj_cover F Γ t b :
-  covered F Γ t ->
-  exists v, (tProj b t) ⤳* v /\ covered (fun Δ u => exists u', u = tProj b u' /\ F Δ u') Γ v.
-Proof.
-  induction 1 as [? t | ??? s * ? ? (bl'&el&?) ? (br'&er&?) |] ; cbn.
-  - exists (tAbort t).
-    split.
-    1: now rewrite ST_Proj_Abort.
+  Lemma ren_covered (F : context -> term -> Prop) (Δ Γ : context) (t : term) (r : ren) :
+    (forall Δ Γ ρ t, F Γ t -> (Δ ⊢ ρ :: Γ) -> F Δ t⟨ρ⟩) ->
+    (Δ ⊢ r :: Γ) ->
+    covered F Γ t ->
+    covered F Δ t⟨r⟩.
+  Proof.
+    intros HF Hren Hcov.
+    induction Hcov in Δ, r, Hren |- * ; cbn ; econstructor ; now eauto with typing.
+  Qed.
+
+  Lemma ren_value (Δ Γ : context) (T : type) (t : term) (r : ren) :
+    value Γ T t ->
+    (Δ ⊢ r :: Γ) ->
+    value Δ T t⟨r⟩.
+  Proof.
+    intros Hval Hren.
+    induction T in Γ, Δ, t, r, Hren, Hval |- * ; cbn in *;
+      try solve [intuition eauto using ren_covered with typing].
+    - split ; [intuition eauto with typing|].
+      intros b.
+      destruct Hval as [_ Hval].
+      specialize (Hval b) as [u Hu].
+      exists (u⟨r⟩).
+      split ; [|now destruct b ; intuition eauto with typing].
+      change (tProj b t⟨r⟩) with ((tProj b t)⟨r⟩).
+      now apply R_ren.
+    - split ; [intuition eauto with typing|].
+      intros Ξ **.
+      edestruct Hval as [_ [v ]].
+      1: eapply ren_comp_typing ; cycle -1 ; eassumption.
+      1: eassumption.
+      exists v.
+      now asimpl ; refold.
+    - eapply ren_covered ; tea.
+      intros ?? r' ? Hval' **.
+      destruct Hval' as [|[[a [->]]|[b [->]]]].
+      + left ; eauto with typing.
+      + right ; left.
+        now exists (a⟨r'⟩).
+      + right ; right.
+        now exists b⟨r'⟩.
+  Qed.
+
+  Lemma sem_ren_subst (Ξ Δ Γ : context) (γ : subst) (r : ren) :
+    (Δ ⊩ γ :: Γ) ->
+    (Ξ ⊢ r :: Δ) ->
+    Ξ ⊩ γ >> ren_term r :: Γ.
+  Proof.
+    intros Hγ ? i **.
+    cbn.
+    now eapply ren_value.
+  Qed.
+
+  (** *** Semantic typing of various substitutions *)
+
+  Lemma sem_Up {Δ Γ : context} {A : type} {γ : subst} : (Δ ⊩ γ :: Γ) -> (Δ,,A) ⊩ ⇑ γ :: (Γ ,, A).
+  Proof.
+    intros Hγ [|] T ? ; cbn in * ; refold.
+    - apply reflect ; eauto with typing.
+    - eapply ren_value ; eauto with typing.
+  Qed.
+
+  Lemma sem_cons (Δ Γ : context) (A : type) (γ : subst) (t : term) :
+    (Δ ⊩ γ :: Γ) ->
+    value Δ A t ->
+    Δ ⊩ t .: γ :: (Γ ,, A).
+  Proof.
+    intros Hγ Ht [|] ? Hin ; cbn.
+    - now inversion Hin ; subst.
+    - now apply Hγ.
+  Qed.
+
+  (** *** We can push eliminators to the leaves of a cover *)
+
+  Lemma proj_cover F Γ t b :
+    covered F Γ t ->
+    exists v, (tProj b t) ⤳* v /\ covered (fun Δ u => exists u', u = tProj b u' /\ F Δ u') Γ v.
+  Proof.
+    induction 1 as [? t | ??? s * ? ? (bl'&el&?) ? (br'&er&?) |] ; cbn.
+    - exists (tAbort t).
+      split.
+      1: now rewrite ST_Proj_Abort.
+      now constructor.
+    - exists (tIf s bl' br').
+      split.
+      1: now rewrite ST_Proj_If, el, er.
+      now econstructor.
+    - exists (tProj b t).
+      split ; [easy|].
+      constructor.
+      now eexists.
+  Qed.
+
+  Lemma app_cover F Γ f t :
+    covered F Γ f ->
+    exists v, (tApp f t) ⤳* v /\
+      covered (fun Δ u => exists u' ρ, (Δ ⊢ ρ :: Γ) /\ u = tApp u' t⟨ρ⟩ /\ F Δ u') Γ v.
+  Proof.
+    intros Hcov.
+    induction Hcov as [? e | ??? s * |? f] in t |- * ; cbn.
+    - exists (tAbort e).
+      split.
+      1: now rewrite ST_App_Abort.
+      now constructor.
+    - specialize (IHHcov1 t⟨↑⟩) as (bl'&el&?).
+      specialize (IHHcov2 t⟨↑⟩) as (br'&er&?).
+      eexists (tIf s bl' br').
+      split.
+      1: now rewrite ST_App_If, el, er.
+      econstructor ; tea.
+      all: eapply map_cover ; tea.
+      all: cbn ; intros ?? (u'&ρ&?&[->]).
+      all: exists u', (↑ >> ρ).
+      all: intuition eauto with typing.
+      all: now asimpl.
+    - exists (tApp f t).
+      split ; [easy|].
+      constructor.
+      eexists _, id.
+      intuition eauto with typing.
+      now asimpl.
+  Qed.
+
+  Lemma abort_cover F Γ t :
+    covered F Γ t ->
+    exists v, (tAbort t) ⤳* v /\ covered (fun Δ u => exists u', u = tAbort u' /\ F Δ u') Γ v.
+  Proof.
+    induction 1 as [? t | ??? s * ? ? (bl'&el&?) ? (br'&er&?) |] ; cbn.
+    - exists (tAbort t).
+      split.
+      1: now rewrite ST_Abort_Abort.
+      now constructor.
+    - exists (tIf s bl' br').
+      split.
+      1: now rewrite ST_Abort_If, el, er.
+      now econstructor.
+    - eexists.
+      split ; [easy|].
+      apply cover_ret.
+      now eexists.
+  Qed.
+
+  Lemma if_cover F Γ s bl br :
+    covered F Γ s ->
+    exists v, (tIf s bl br) ⤳* v /\
+      covered (fun Δ u => exists u' ρ, (Δ ⊢ ρ :: Γ) /\ u = tIf u' bl⟨⇑ ρ⟩ br⟨⇑ ρ⟩ /\ F Δ u') Γ v.
+  Proof.
+    intros Hcov.
+    induction Hcov as [? e | ??? s * |? s] in bl, br |- * ; cbn.
+    - exists (tAbort e).
+      split.
+      1: now rewrite ST_If_Abort.
+      now constructor.
+    - specialize (IHHcov1 bl⟨⇑ ↑⟩ br⟨⇑ ↑⟩) as (bl'&el&?).
+      specialize (IHHcov2 bl⟨⇑ ↑⟩ br⟨⇑ ↑⟩) as (br'&er&?).
+      eexists (tIf s bl' br').
+      split.
+      1: now rewrite ST_If_If, el, er.
+      econstructor ; tea.
+      all: eapply map_cover ; tea.
+      all: cbn ; intros ?? (u'&ρ&?&[->]).
+      all: exists u', (↑ >> ρ).
+      all: intuition eauto with typing.
+      all: now rewrite !up_up_ren.
+    - exists (tIf s bl br).
+      split ; [easy|].
+      constructor.
+      eexists _, id.
+      intuition eauto with typing.
+      now rewrite !up_id.
+  Qed.
+
+  (** *** Covering and reducibility *)
+
+  (** A term covered by reducible term reduces to a term covered by values, by
+    reducing all leaves *)
+  Lemma covered_red Γ T t :
+    covered (fun Δ u => reducible Δ T u) Γ t ->
+    exists t', t ⤳* t' /\ covered (fun Δ u => value Δ T u) Γ t'.
+  Proof.
+    induction 1 as [? t | ??? s * ? ? (bl'&?&?) ? (br'&?&?)|? ? [t']].
+    - exists (tAbort t).
+      split ; [easy|].
+      now constructor.
+    - exists (tIf s bl' br').
+      split ; [now rewrite R_If_cong|].
+      now econstructor.
+    - exists t' ; split ; [easy|].
+      now constructor.
+  Qed.
+
+  (** A term covered by values is reducible
+    Proven by induction on the type, if it is positive we are essentially done,
+    otherwise we push observations to the leaves thanks to the above lemmas. *)
+  Lemma cover_value Γ T t :
+    covered (fun Δ u => value Δ T u) Γ t ->
+    reducible Γ T t.
+  Proof.
+    intros Hcov.
+    induction T in Γ, T , t , Hcov |- *.
+    all: try solve [now exists t ; cbn ; eauto using join_cover].
+    - apply value_red ; cbn.
+      apply covered_nf.
+      eapply map_cover ; tea.
+      now cbn.
+    - apply value_red ; cbn.
+      split.
+      + eapply covered_nf, map_cover ; tea.
+        cbn ; easy.
+      + intros b.
+        eapply proj_cover in Hcov as [t' []] ; cbn in *.
+        eapply red_antired ; tea.
+        edestruct (covered_red Γ (if b then T1 else T2) t') as (t''&?&?).
+        1:{ 
+          eapply map_cover ; [..|eassumption].
+          cbn.
+          now intros ?? (?&->&[_ Hred]).
+        }
+        destruct b ; now eapply red_antired.
+    - apply value_red ; cbn.
+      split.
+      + eapply covered_nf, map_cover ; tea.
+        cbn ; easy.
+      + intros Δ u ρ Hρ Hred.
+        eapply ren_covered in Hcov ; tea.
+        2: now eauto using ren_value.
+        apply (app_cover _ _ _ u) in Hcov as [t' []] ; cbn in *.
+        eapply red_antired ; tea.
+        edestruct (covered_red Δ T2 t') as (t''&?&?).
+        1:{ 
+          eapply map_cover ; [..|eassumption].
+          cbn.
+          intros ?? (f&?&?&->&[_ Hred']).
+          replace f with f⟨id⟩ by now asimpl.
+          apply Hred' ; eauto with typing.
+          now eapply ren_value.
+        }
+        now eapply red_antired.
+  Qed.
+
+  (** Any term covered by reducible terms is reducible *)
+  Lemma cover_reducible Γ T t :
+    covered (fun Δ u => reducible Δ T u) Γ t ->
+    reducible Γ T t.
+  Proof.
+    intros (?&?&?)%covered_red.
+    eauto using red_antired, cover_value.
+  Qed.
+
+  (** *** Semantic typing lemmas *)
+
+  Lemma sem_Const Γ c :
+    Γ ⊩ tConst c :: const_type c.
+  Proof.
+    intros Δ γ Hγ.
+    cbn.
+    apply value_red, reflect.
     now constructor.
-  - exists (tIf s bl' br').
-    split.
-    1: now rewrite ST_Proj_If, el, er.
+  Qed.
+
+  Lemma sem_Var n Γ T :
+    in_context n Γ T ->
+    Γ ⊩ tVar n :: T.
+  Proof.
+    intros Hin Δ γ Hγ.
+    specialize (Hγ _ _ Hin).
+    now apply value_red.
+  Qed.
+
+  Lemma sem_Star Γ :
+    Γ ⊩ tStar :: TUnit.
+  Proof.
+    intros ? ** ; cbn.
+    apply value_red ; cbn.
     now econstructor.
-  - exists (tProj b t).
-    split ; [easy|].
-    constructor.
-    now eexists.
-Qed.
+  Qed.
 
-Lemma app_cover F Γ f t :
-  covered F Γ f ->
-  exists v, (tApp f t) ⤳* v /\
-    covered (fun Δ u => exists u' ρ, (Δ ⊢ ρ :: Γ) /\ u = tApp u' t⟨ρ⟩ /\ F Δ u') Γ v.
-Proof.
-  intros Hcov.
-  induction Hcov as [? e | ??? s * |? f] in t |- * ; cbn.
-  - exists (tAbort e).
+  Lemma sem_App Γ A B f u :
+    (Γ ⊩ f :: TFun A B) ->
+    (Γ ⊩ u :: A) ->
+    Γ ⊩ tApp f u :: B.
+  Proof.
+    intros Hf Hu Δ γ Hγ.
+    cbn.
+    destruct (Hf _ γ Hγ) as [f' (Hredf&?&Hf')].
+    destruct (Hu _ γ Hγ) as [u' [Hredu]].
+    cbn in *.
+    apply (red_antired (tApp f' u')).
+    - replace f' with (f'⟨ids⟩) by (now asimpl).
+      apply Hf'.
+      all: now eauto with typing.
+    - now rewrite Hredf, Hredu.
+  Qed.
+
+  Lemma sem_Pair Γ A B a b :
+    (Γ ⊩ a :: A) ->
+    (Γ ⊩ b :: B) ->
+    (Γ ⊩ tPair a b :: TProd A B).
+  Proof.
+    intros Ha Hb Δ γ Hγ.
+    destruct (Ha _ γ Hγ) as [a' [Hreda]].
+    destruct (Hb _ γ Hγ) as [b' [Hredb]].
+    exists (tPair a' b').
+    split ; [|split] ; cbn.
+    - now rewrite Hreda, Hredb.
+    - auto using reify with typing.
+    - intros [].
+      all: eapply red_antired ; [now apply value_red|].
+      all: now rewrite ?ST_Fst, ?ST_Snd.
+  Qed.
+
+  Lemma sem_Fst Γ A B t :
+    (Γ ⊩ t :: TProd A B) ->
+    (Γ ⊩ tFst t :: A).
+  Proof.
+    intros Ht Δ γ Hγ.
+    specialize (Ht _ _ Hγ) as [t' [Hred [? IH]]] ; cbn in *.
+    apply (red_antired (tFst t')).
+    2: now rewrite Hred.
+    now specialize (IH true).
+  Qed.
+
+  Lemma sem_Snd Γ A B t :
+    (Γ ⊩ t :: TProd A B) ->
+    (Γ ⊩ tSnd t :: B).
+  Proof.
+    intros Ht Δ γ Hγ.
+    specialize (Ht _ _ Hγ) as [t' [Hred [? IH]]] ; cbn in *.
+    apply (red_antired (tSnd t')).
+    2: now rewrite Hred.
+    now specialize (IH false).
+  Qed.
+
+  Lemma sem_Lam Γ A B t :
+    (Γ ,, A ⊩ t :: B) ->
+    Γ ⊩ tLam t :: TFun A B.
+  Proof.
+    intros Ht Δ γ Hγ.
+    cbn ; refold.
+    edestruct (Ht (Δ,,A) (⇑ γ)) as [t' [Hred]].
+    1: now eapply sem_Up.
+    exists (tLam t').
+    split ; [now rewrite Hred|].
+    cbn.
     split.
-    1: now rewrite ST_App_Abort.
+    1: now eauto using reify with typing.
+    intros Ξ v ** ; refold.
+    eapply red_antired.
+    2: now rewrite ST_Beta_Fun.
+    edestruct (Ht Ξ) as [v' [Hred']].
+    1:{
+      apply sem_cons ; [|eassumption].
+      now eapply sem_ren_subst.
+    }
+    exists v' ; split ; [|easy].
+    replace (t[_]) with (t[⇑ γ]⟨⇑ ρ⟩[v..]) in Hred'
+      by (substify ; now asimpl).
+    assert (t[⇑ γ]⟨⇑ ρ⟩[v..] ⤳* t'⟨⇑ ρ⟩ [v..]) as Hred''
+      by now rewrite Hred.
+    eapply confluence in Hred'' as (v''&?&?).
+    2: exact Hred'.
+    enough (v' = v'') as -> by easy.
+    eapply nf_red_eq ; tea.
+    now apply reify.
+  Qed.
+
+  Lemma sem_Abort Γ A t :
+    (Γ ⊩ t :: TEmp) ->
+    (Γ ⊩ tAbort t :: A).
+  Proof.
+    intros Ht Δ γ Hγ.
+    specialize (Ht _ _ Hγ) as [t' [Hred Hne]] ; cbn in *.
+    eapply abort_cover in Hne as (t''&Hred'&?).
+    eapply red_antired.
+    2: now rewrite Hred, Hred'.
+    eapply cover_reducible, map_cover ; tea.
+    intros ?? (?&->&?).
+    eapply cover_reducible.
     now constructor.
-  - specialize (IHHcov1 t⟨↑⟩) as (bl'&el&?).
-    specialize (IHHcov2 t⟨↑⟩) as (br'&er&?).
-    eexists (tIf s bl' br').
-    split.
-    1: now rewrite ST_App_If, el, er.
-    econstructor ; tea.
-    all: eapply map_cover ; tea.
-    all: cbn ; intros ?? (u'&ρ&?&[->]).
-    all: exists u', (↑ >> ρ).
-    all: intuition eauto with typing.
-    all: now asimpl.
-  - exists (tApp f t).
-    split ; [easy|].
+  Qed.
+
+  Lemma sem_Left Γ A B t :
+    (Γ ⊩ t :: A) ->
+    (Γ ⊩ tLeft t :: TSum A B).
+  Proof.
+    intros Ht Δ γ Hγ.
+    specialize (Ht _ _ Hγ) as [t' [Hred Hval]] ; cbn in *.
+    exists (tLeft t').
+    split ; [now rewrite Hred|].
     constructor.
-    eexists _, id.
-    intuition eauto with typing.
+    right ; left.
+    now eexists.
+  Qed.
+
+  Lemma sem_Right Γ A B t :
+    (Γ ⊩ t :: B) ->
+    (Γ ⊩ tRight t :: TSum A B).
+  Proof.
+    intros Ht Δ γ Hγ.
+    specialize (Ht _ _ Hγ) as [t' [Hred Hval]] ; cbn in *.
+    exists (tRight t').
+    split ; [now rewrite Hred|].
+    constructor.
+    right ; right.
+    now eexists.
+  Qed.
+
+  Lemma sem_If Γ A B T s bl br :
+    (Γ ⊩ s :: TSum A B) ->
+    (Γ,,A ⊩ bl :: T) ->
+    (Γ,,B ⊩ br :: T) ->
+    (Γ ⊩ tIf s bl br :: T).
+  Proof.
+    intros Hs Hl Hr Δ γ Hγ.
+    specialize (Hs _ _ Hγ) as [s' [Hred Hne]] ; cbn in *.
+    eapply if_cover in Hne as (t''&Hred'&?).
+    eapply red_antired.
+    2: now rewrite Hred, Hred'.
+    eapply cover_reducible, map_cover ; tea.
+    intros Δ' ? (?&ρ&?&->&Hval).
+    eapply cover_reducible.
+    constructor.
+    destruct Hval as [| [(a&->&?)|(b&->&?)]].
+    - eapply cover_reducible.
+      rewrite !up_up_subst_ren.
+      econstructor ; tea.
+      all: constructor.
+      + now eapply Hl, sem_Up, sem_ren_subst.
+      + now eapply Hr, sem_Up, sem_ren_subst.
+    - eapply red_antired.
+      2: now rewrite ST_Left.
+      replace (_[_..]) with (bl[a .: (γ >> ren_term ρ)]).
+      2:{ substify ; asimpl ; refold.
+          apply subst_term_morphism ; [|easy].
+          intros [|] ; cbn ; [easy|].
+          apply subst_term_morphism ; [|easy].
+          now intros [|].
+      }
+      eapply Hl, sem_cons.
+      2: assumption.
+      now eapply sem_ren_subst.
+    - eapply red_antired.
+      2: now rewrite ST_Right.
+      replace (_[_..]) with (br[b .: (γ >> ren_term ρ)]).
+      2:{ substify ; asimpl ; refold.
+          apply subst_term_morphism ; [|easy].
+          intros [|] ; cbn ; [easy|].
+          apply subst_term_morphism ; [|easy].
+          now intros [|].
+      }
+      eapply Hr, sem_cons.
+      2: assumption.
+      now eapply sem_ren_subst.
+  Qed.
+
+  (** *** The fundamental lemma: typing implies semantic typing *)
+
+  Theorem fundamental Γ T (t : term) :
+    (Γ ⊢ t :: T) ->
+    (Γ ⊩ t :: T).
+  Proof.
+    intros Hty.
+    induction Hty.
+    - now apply sem_Const.
+    - now apply sem_Var.
+    - now apply sem_Star.
+    - now apply sem_Lam.
+    - now eapply sem_App.
+    - now eapply sem_Pair.
+    - now eapply sem_Fst.
+    - now eapply sem_Snd.
+    - now eapply sem_Abort.
+    - now eapply sem_Left.
+    - now eapply sem_Right.
+    - now eapply sem_If.
+  Qed.
+
+  (** We conclude by using the above with the identity substitution *)
+  Lemma sem_id (Γ : context) : (Γ ⊩ ids :: Γ).
+  Proof.
+    intros i ** ; cbn.
+    apply reflect.
+    eauto with typing.
+  Qed.
+
+  Corollary sem_red (Γ : context) (A : type) (t : term) : (Γ ⊩ t :: A) -> reducible Γ A t.
+  Proof.
+    intros Ht.
+    specialize (Ht Γ ids (sem_id _)).
+    enough (t[ids] = t) as [] by easy.
     now asimpl.
-Qed.
+  Qed.
 
-Lemma abort_cover F Γ t :
-  covered F Γ t ->
-  exists v, (tAbort t) ⤳* v /\ covered (fun Δ u => exists u', u = tAbort u' /\ F Δ u') Γ v.
-Proof.
-  induction 1 as [? t | ??? s * ? ? (bl'&el&?) ? (br'&er&?) |] ; cbn.
-  - exists (tAbort t).
-    split.
-    1: now rewrite ST_Abort_Abort.
-    now constructor.
-  - exists (tIf s bl' br').
-    split.
-    1: now rewrite ST_Abort_If, el, er.
-    now econstructor.
-  - eexists.
-    split ; [easy|].
-    apply cover_ret.
-    now eexists.
-Qed.
+  Corollary normalisation Γ T (t : term) :
+    (Γ ⊢ t :: T) ->
+    exists u, (t ⤳* u) /\ (Γ ⊢ u ◃ T).
+  Proof.
+    intros []%fundamental%sem_red.
+    eexists ; split ; intuition eauto using reify.
+  Qed.
 
-Lemma if_cover F Γ s bl br :
-  covered F Γ s ->
-  exists v, (tIf s bl br) ⤳* v /\
-    covered (fun Δ u => exists u' ρ, (Δ ⊢ ρ :: Γ) /\ u = tIf u' bl⟨⇑ ρ⟩ br⟨⇑ ρ⟩ /\ F Δ u') Γ v.
-Proof.
-  intros Hcov.
-  induction Hcov as [? e | ??? s * |? s] in bl, br |- * ; cbn.
-  - exists (tAbort e).
-    split.
-    1: now rewrite ST_If_Abort.
-    now constructor.
-  - specialize (IHHcov1 bl⟨⇑ ↑⟩ br⟨⇑ ↑⟩) as (bl'&el&?).
-    specialize (IHHcov2 bl⟨⇑ ↑⟩ br⟨⇑ ↑⟩) as (br'&er&?).
-    eexists (tIf s bl' br').
-    split.
-    1: now rewrite ST_If_If, el, er.
-    econstructor ; tea.
-    all: eapply map_cover ; tea.
-    all: cbn ; intros ?? (u'&ρ&?&[->]).
-    all: exists u', (↑ >> ρ).
-    all: intuition eauto with typing.
-    all: now rewrite !up_up_ren.
-  - exists (tIf s bl br).
-    split ; [easy|].
-    constructor.
-    eexists _, id.
-    intuition eauto with typing.
-    now rewrite !up_id.
-Qed.
-
-(** *** Covering and reducibility *)
-
-(** A term covered by reducible term reduces to a term covered by values, by
-  reducing all leaves *)
-Lemma covered_red Γ T t :
-  covered (fun Δ u => reducible Δ T u) Γ t ->
-  exists t', t ⤳* t' /\ covered (fun Δ u => value Δ T u) Γ t'.
-Proof.
-  induction 1 as [? t | ??? s * ? ? (bl'&?&?) ? (br'&?&?)|? ? [t']].
-  - exists (tAbort t).
-    split ; [easy|].
-    now constructor.
-  - exists (tIf s bl' br').
-    split ; [now rewrite R_If_cong|].
-    now econstructor.
-  - exists t' ; split ; [easy|].
-    now constructor.
-Qed.
-
-(** A term covered by values is reducible
-  Proven by induction on the type, if it is positive we are essentially done,
-  otherwise we push observations to the leaves thanks to the above lemmas. *)
-Lemma cover_value Γ T t :
-  covered (fun Δ u => value Δ T u) Γ t ->
-  reducible Γ T t.
-Proof.
-  intros Hcov.
-  induction T in Γ, T , t , Hcov |- *.
-  all: try solve [now exists t ; cbn ; eauto using join_cover].
-  - apply value_red ; cbn.
-    apply covered_nf.
-    eapply map_cover ; tea.
-    now cbn.
-  - apply value_red ; cbn.
-    split.
-    + eapply covered_nf, map_cover ; tea.
-      cbn ; easy.
-    + intros b.
-      eapply proj_cover in Hcov as [t' []] ; cbn in *.
-      eapply red_antired ; tea.
-      edestruct (covered_red Γ (if b then T1 else T2) t') as (t''&?&?).
-      1:{ 
-        eapply map_cover ; [..|eassumption].
-        cbn.
-        now intros ?? (?&->&[_ Hred]).
-      }
-      destruct b ; now eapply red_antired.
-  - apply value_red ; cbn.
-    split.
-    + eapply covered_nf, map_cover ; tea.
-      cbn ; easy.
-    + intros Δ u ρ Hρ Hred.
-      eapply ren_covered in Hcov ; tea.
-      2: now eauto using ren_value.
-      apply (app_cover _ _ _ u) in Hcov as [t' []] ; cbn in *.
-      eapply red_antired ; tea.
-      edestruct (covered_red Δ T2 t') as (t''&?&?).
-      1:{ 
-        eapply map_cover ; [..|eassumption].
-        cbn.
-        intros ?? (f&?&?&->&[_ Hred']).
-        replace f with f⟨id⟩ by now asimpl.
-        apply Hred' ; eauto with typing.
-        now eapply ren_value.
-      }
-      now eapply red_antired.
-Qed.
-
-(** Any term covered by reducible terms is reducible *)
-Lemma cover_reducible Γ T t :
-  covered (fun Δ u => reducible Δ T u) Γ t ->
-  reducible Γ T t.
-Proof.
-  intros (?&?&?)%covered_red.
-  eauto using red_antired, cover_value.
-Qed.
-
-(** *** Semantic typing lemmas *)
-
-Lemma sem_Var n Γ T :
-  in_context n Γ T ->
-  Γ ⊩ tVar n :: T.
-Proof.
-  intros Hin Δ γ Hγ.
-  specialize (Hγ _ _ Hin).
-  now apply value_red.
-Qed.
-
-Lemma sem_Star Γ :
-  Γ ⊩ tStar :: TUnit.
-Proof.
-  intros ? ** ; cbn.
-  apply value_red ; cbn.
-  now econstructor.
-Qed.
-
-Lemma sem_App Γ A B f u :
-  (Γ ⊩ f :: TFun A B) ->
-  (Γ ⊩ u :: A) ->
-  Γ ⊩ tApp f u :: B.
-Proof.
-  intros Hf Hu Δ γ Hγ.
-  cbn.
-  destruct (Hf _ γ Hγ) as [f' (Hredf&?&Hf')].
-  destruct (Hu _ γ Hγ) as [u' [Hredu]].
-  cbn in *.
-  apply (red_antired (tApp f' u')).
-  - replace f' with (f'⟨ids⟩) by (now asimpl).
-    apply Hf'.
-    all: now eauto with typing.
-  - now rewrite Hredf, Hredu.
-Qed.
-
-Lemma sem_Pair Γ A B a b :
-  (Γ ⊩ a :: A) ->
-  (Γ ⊩ b :: B) ->
-  (Γ ⊩ tPair a b :: TProd A B).
-Proof.
-  intros Ha Hb Δ γ Hγ.
-  destruct (Ha _ γ Hγ) as [a' [Hreda]].
-  destruct (Hb _ γ Hγ) as [b' [Hredb]].
-  exists (tPair a' b').
-  split ; [|split] ; cbn.
-  - now rewrite Hreda, Hredb.
-  - auto using reify with typing.
-  - intros [].
-    all: eapply red_antired ; [now apply value_red|].
-    all: now rewrite ?ST_Fst, ?ST_Snd.
-Qed.
-
-Lemma sem_Fst Γ A B t :
-  (Γ ⊩ t :: TProd A B) ->
-  (Γ ⊩ tFst t :: A).
-Proof.
-  intros Ht Δ γ Hγ.
-  specialize (Ht _ _ Hγ) as [t' [Hred [? IH]]] ; cbn in *.
-  apply (red_antired (tFst t')).
-  2: now rewrite Hred.
-  now specialize (IH true).
-Qed.
-
-Lemma sem_Snd Γ A B t :
-  (Γ ⊩ t :: TProd A B) ->
-  (Γ ⊩ tSnd t :: B).
-Proof.
-  intros Ht Δ γ Hγ.
-  specialize (Ht _ _ Hγ) as [t' [Hred [? IH]]] ; cbn in *.
-  apply (red_antired (tSnd t')).
-  2: now rewrite Hred.
-  now specialize (IH false).
-Qed.
-
-Lemma sem_Lam Γ A B t :
-  (Γ ,, A ⊩ t :: B) ->
-  Γ ⊩ tLam t :: TFun A B.
-Proof.
-  intros Ht Δ γ Hγ.
-  cbn ; refold.
-  edestruct (Ht (Δ,,A) (⇑ γ)) as [t' [Hred]].
-  1: now eapply sem_Up.
-  exists (tLam t').
-  split ; [now rewrite Hred|].
-  cbn.
-  split.
-  1: now eauto using reify with typing.
-  intros Ξ v ** ; refold.
-  eapply red_antired.
-  2: now rewrite ST_Beta_Fun.
-  edestruct (Ht Ξ) as [v' [Hred']].
-  1:{
-    apply sem_cons ; [|eassumption].
-    now eapply sem_ren_subst.
-  }
-  exists v' ; split ; [|easy].
-  replace (t[_]) with (t[⇑ γ]⟨⇑ ρ⟩[v..]) in Hred'
-    by (substify ; now asimpl).
-  assert (t[⇑ γ]⟨⇑ ρ⟩[v..] ⤳* t'⟨⇑ ρ⟩ [v..])
-    by now rewrite Hred.
-  (* confluence *)
-Admitted.
-
-Lemma sem_Abort Γ A t :
-  (Γ ⊩ t :: TEmp) ->
-  (Γ ⊩ tAbort t :: A).
-Proof.
-  intros Ht Δ γ Hγ.
-  specialize (Ht _ _ Hγ) as [t' [Hred Hne]] ; cbn in *.
-  eapply abort_cover in Hne as (t''&Hred'&?).
-  eapply red_antired.
-  2: now rewrite Hred, Hred'.
-  eapply cover_reducible, map_cover ; tea.
-  intros ?? (?&->&?).
-  eapply cover_reducible.
-  now constructor.
-Qed.
-
-Lemma sem_Left Γ A B t :
-  (Γ ⊩ t :: A) ->
-  (Γ ⊩ tLeft t :: TSum A B).
-Proof.
-  intros Ht Δ γ Hγ.
-  specialize (Ht _ _ Hγ) as [t' [Hred Hval]] ; cbn in *.
-  exists (tLeft t').
-  split ; [now rewrite Hred|].
-  constructor.
-  right ; left.
-  now eexists.
-Qed.
-
-Lemma sem_Right Γ A B t :
-  (Γ ⊩ t :: B) ->
-  (Γ ⊩ tRight t :: TSum A B).
-Proof.
-  intros Ht Δ γ Hγ.
-  specialize (Ht _ _ Hγ) as [t' [Hred Hval]] ; cbn in *.
-  exists (tRight t').
-  split ; [now rewrite Hred|].
-  constructor.
-  right ; right.
-  now eexists.
-Qed.
-
-Lemma sem_If Γ A B T s bl br :
-  (Γ ⊩ s :: TSum A B) ->
-  (Γ,,A ⊩ bl :: T) ->
-  (Γ,,B ⊩ br :: T) ->
-  (Γ ⊩ tIf s bl br :: T).
-Proof.
-  intros Hs Hl Hr Δ γ Hγ.
-  specialize (Hs _ _ Hγ) as [s' [Hred Hne]] ; cbn in *.
-  eapply if_cover in Hne as (t''&Hred'&?).
-  eapply red_antired.
-  2: now rewrite Hred, Hred'.
-  eapply cover_reducible, map_cover ; tea.
-  intros Δ' ? (?&ρ&?&->&Hval).
-  eapply cover_reducible.
-  constructor.
-  destruct Hval as [| [(a&->&?)|(b&->&?)]].
-  - eapply cover_reducible.
-    rewrite !up_up_subst_ren.
-    econstructor ; tea.
-    all: constructor.
-    + now eapply Hl, sem_Up, sem_ren_subst.
-    + now eapply Hr, sem_Up, sem_ren_subst.
-  - eapply red_antired.
-    2: now rewrite ST_Left.
-    replace (_[_..]) with (bl[a .: (γ >> ren_term ρ)]).
-    2:{ substify ; asimpl ; refold.
-        apply subst_term_morphism ; [|easy].
-        intros [|] ; cbn ; [easy|].
-        apply subst_term_morphism ; [|easy].
-        now intros [|].
-    }
-    eapply Hl, sem_cons.
-    2: assumption.
-    now eapply sem_ren_subst.
-  - eapply red_antired.
-    2: now rewrite ST_Right.
-    replace (_[_..]) with (br[b .: (γ >> ren_term ρ)]).
-    2:{ substify ; asimpl ; refold.
-        apply subst_term_morphism ; [|easy].
-        intros [|] ; cbn ; [easy|].
-        apply subst_term_morphism ; [|easy].
-        now intros [|].
-    }
-    eapply Hr, sem_cons.
-    2: assumption.
-    now eapply sem_ren_subst.
-Qed.
-
-(** *** The fundamental lemma: typing implies semantic typing *)
-
-Theorem fundamental Γ T (t : term) :
-  (Γ ⊢ t :: T) ->
-  (Γ ⊩ t :: T).
-Proof.
-  intros Hty.
-  induction Hty.
-  - now apply sem_Const.
-  - now apply sem_Var.
-  - now apply sem_Star.
-  - now apply sem_Lam.
-  - now eapply sem_App.
-  - now eapply sem_Pair.
-  - now eapply sem_Fst.
-  - now eapply sem_Snd.
-  - now eapply sem_Abort.
-  - now eapply sem_Left.
-  - now eapply sem_Right.
-  - now eapply sem_If.
-Qed.
-
-(** We conclude by using the above with the identity substitution *)
-Lemma sem_id (Γ : context) : (Γ ⊩ ids :: Γ).
-Proof.
-  intros i ** ; cbn.
-  apply reflect.
-  eauto with typing.
-Qed.
-
-Corollary sem_red (Γ : context) (A : type) (t : term) : (Γ ⊩ t :: A) -> reducible Γ A t.
-Proof.
-  intros Ht.
-  specialize (Ht Γ ids (sem_id _)).
-  enough (t[ids] = t) as [] by easy.
-  now asimpl.
-Qed.
-
-Corollary normalisation Γ T (t : term) :
-  (Γ ⊢ t :: T) ->
-  exists u, (t ⤳* u) /\ (Γ ⊢ u ◃ T).
-Proof.
-  intros []%fundamental%sem_red.
-  eexists ; split ; intuition eauto using reify.
-Qed.
+End Normalisation.
