code/theories/Syntax.v
@@ -1,8 +1,8 @@
 From smpl Require Import Smpl.
-From Stdlib Require Import ssrbool List.
+From Stdlib Require Import List.
 From Stdlib Require Import Setoid Morphisms Relation_Definitions RelationClasses.
-From Interpolation Require Export BasicAst core unscoped Ast Context.
 From Interpolation Require Import Utils.
+From Interpolation Require Export BasicAst core unscoped Ast Context.
 
 (* Export UnscopedNotations.
 #[global] Open Scope subst_scope. *)
@@ -26,11 +26,9 @@ Notation "s ⟨ xi1 ⟩" := (ren1 xi1 s) (at level 7, left associativity, format
 
 Notation "s [ sigma ]" := (subst1 sigma s) (at level 7, left associativity, format "s '/' [ sigma ]") : asubst_scope.
 
-Notation "s [ t ]⇑" := (subst_term (scons t (shift >> ids)) s) (at level 7, left associativity, format "s '/' [ t ]⇑") : asubst_scope.
-
 Notation "s '..'" := (scons s ids) (at level 1, format "s ..") : asubst_scope.
 
-Notation "↑" := (shift) : asubst_scope.
+Notation "↑" := (unscoped.shift) : asubst_scope.
 
 Notation "⇑ σ" := (up_term σ) (at level 1) : asubst_scope.
 
@@ -47,7 +45,8 @@ Notation "'eSnd'" := (eProj false).
 Notation "'tLeft'" := (tIn false).
 Notation "'tRight'" := (tIn true).
 
-#[global] Instance Ren_elim : (Ren1 (nat -> nat) elim elim) := fun ρ e => @subst_elim (ρ >> tVar) e.
+#[global] Instance Ren_elim `{Lang} : (Ren1 (nat -> nat) elim elim) :=
+  fun ρ e => @subst_elim _ _ (ρ >> tVar) e.
 
 #[global] Instance Ren1_subst {Y Z : Type} `{Ren1 (nat -> nat) Y Z} :
   (Ren1 (nat -> nat) (nat -> Y) (nat -> Z)) :=
@@ -80,124 +79,158 @@ Arguments VarInstance_term _/.
 
 (** ** Lemmas *)
 
-Lemma up_up_ren ρ ρ' (t : term) : t⟨⇑ ρ⟩⟨⇑ ρ'⟩ = t⟨⇑ (ρ >> ρ')⟩.
-Proof.
-  substify ; asimpl ; refold.
-  apply subst_term_morphism.
-  1: now intros [|].
-  easy.
-Qed.
+Section Lemmas.
+Context `{Lang}.
 
-Lemma up_up_subst_ren (σ : subst) (ρ : ren) (t : term) :
-  t[⇑ σ]⟨⇑ ρ⟩ = t[⇑ (σ >> ren_term ρ)].
-Proof.
-  substify ; asimpl ; refold.
-  apply subst_term_morphism.
-  2: easy.
-  intros [|] ; cbn ; refold ; try easy.
-  substify ; refold.
-  apply subst_term_morphism.
-  2: easy.
-  now intros [|].
-Qed.
+  Lemma subst_id (σ : subst) (t : term) : σ =1 ids -> t[σ] = t.
+  Proof.
+    intros Hσ.
+    unfold subst1, Subst_term.
+    erewrite ext_term ; tea.
+    now asimpl.
+  Qed.
 
-Lemma up_id (t : term) : t⟨⇑ id⟩ = t.
-Proof.
-  rewrite ren_term_morphism.
-  1: apply rinstId'_term.
-  1: now intros [|].
-  easy.
-Qed.
+  Lemma renRen_term (ρ ρ' : ren) (t : term) : t⟨ρ⟩⟨ρ'⟩ = t⟨ρ >> ρ'⟩.
+  Proof.
+    apply renRen_term.
+  Qed.
 
-Lemma subst1_ren (t u : term) (ρ : ren) : t[u..]⟨ρ⟩ = t⟨⇑ ρ⟩[u⟨ρ⟩..].
-Proof.
-  now substify ; asimpl.
-Qed.
+  Lemma up_up_ren ρ ρ' (t : term) : t⟨⇑ ρ⟩⟨⇑ ρ'⟩ = t⟨⇑ (ρ >> ρ')⟩.
+  Proof.
+    substify ; asimpl ; refold.
+    apply subst_term_morphism.
+    1: now intros [|].
+    easy.
+  Qed.
 
-Lemma subst1_subst (t u : term) (σ : subst) : t[u..][σ] = t[⇑ σ][u[σ]..].
-Proof.
-  now asimpl.
-Qed.
+  Lemma up_up_subst_ren (σ : subst) (ρ : ren) (t : term) :
+    t[⇑ σ]⟨⇑ ρ⟩ = t[⇑ (σ >> ren_term ρ)].
+  Proof.
+    substify ; asimpl ; refold.
+    apply subst_term_morphism.
+    2: easy.
+    intros [|] ; cbn ; refold ; try easy.
+    substify ; refold.
+    apply subst_term_morphism.
+    2: easy.
+    now intros [|].
+  Qed.
 
-Lemma up_lift_ren (t : term) ρ : t⟨↑⟩⟨⇑ ρ⟩ = t⟨ρ⟩⟨↑⟩.
-Proof.
-  now asimpl.
-Qed.
+  Lemma up_id (t : term) : t⟨⇑ id⟩ = t.
+  Proof.
+    enough (⇑ id =1 id) as e by 
+      (rewrite e ; now asimpl).
+    now intros [|].
+  Qed.
 
-Lemma up_lift_up_ren (t : term) ρ : t⟨⇑ ↑⟩⟨⇑ (⇑ ρ)⟩ = t⟨⇑ ρ⟩⟨⇑ ↑⟩.
-Proof.
-  intros ; asimpl ; refold.
-  apply ren_term_morphism ; [|reflexivity].
-  intros [|] ; reflexivity.
-Qed.
+  Lemma subst1_ren (t u : term) (ρ : ren) : t[u..]⟨ρ⟩ = t⟨⇑ ρ⟩[u⟨ρ⟩..].
+  Proof.
+    now substify ; asimpl.
+  Qed.
 
-Lemma up_lift_subst (t : term) σ : t⟨↑⟩[⇑ σ] = t[σ]⟨↑⟩.
-Proof.
-  now asimpl.
-Qed.
+  Lemma subst1_subst (t u : term) (σ : subst) : t[u..][σ] = t[⇑ σ][u[σ]..].
+  Proof.
+    now asimpl.
+  Qed.
 
-Lemma up_lift_up_subst (t : term) σ : t⟨⇑ ↑⟩[⇑ (⇑ σ)] = t[⇑ σ]⟨⇑ ↑⟩.
-Proof.
-  intros ; asimpl ; refold.
-  apply subst_term_morphism ; [|reflexivity].
-  intros [|] ; reflexivity.
-Qed.
+  Lemma up_lift_ren (t : term) (ρ : ren) : t⟨↑⟩⟨⇑ ρ⟩ = t⟨ρ⟩⟨↑⟩.
+  Proof.
+    now asimpl.
+  Qed.
 
-Lemma elim_ren (e : elim) ρ : e⟨ρ⟩ = e[ρ >> tVar].
-Proof.
-  substify ; refold.
-  reflexivity.
-Qed.
+  Lemma up_lift_up_ren (t : term) ρ : t⟨⇑ ↑⟩⟨⇑ (⇑ ρ)⟩ = t⟨⇑ ρ⟩⟨⇑ ↑⟩.
+  Proof.
+    intros ; asimpl ; refold.
+    apply ren_term_morphism ; [|reflexivity].
+    intros [|] ; reflexivity.
+  Qed.
 
-Definition tip (f : term -> term) : subst :=  (f (tVar 0)).: (↑ >> ids).
+  Lemma up_lift_subst (t : term) σ : t⟨↑⟩[⇑ σ] = t[σ]⟨↑⟩.
+  Proof.
+    now asimpl.
+  Qed.
 
-Lemma tip_subst (f : term -> term) (t u : term) :
-  (forall σ x, (f x) [σ] = f (x[σ])) ->
-  u[tip f][t ..] = u[(f t)..].
-Proof.
-  intros Hf.
-  rewrite substSubst_term ; refold.
-  apply ext_term.
-  intros x.
-  unfold tip.
-  asimpl ; cbn.
-  destruct x ; cbn ; [|easy].
-  rewrite Hf ; asimpl.
-  reflexivity.
-Qed.
+  Lemma up_lift_up_subst (t : term) σ : t⟨⇑ ↑⟩[⇑ (⇑ σ)] = t[⇑ σ]⟨⇑ ↑⟩.
+  Proof.
+    intros ; asimpl ; refold.
+    apply subst_term_morphism ; [|reflexivity].
+    intros [|] ; reflexivity.
+  Qed.
 
-Lemma tip_shift (f : term -> term) ρ (t : term) :
-  (forall σ x, (f x) [σ] = f (x[σ])) ->
-  t[tip f]⟨⇑ ρ⟩ = t⟨⇑ ρ⟩[tip f].
-Proof.
-  intros Hf.
-  unfold tip.
-  substify ; asimpl.
-  rewrite Hf ; asimpl.
-  reflexivity.
-Qed.
+  Lemma elim_ren (e : elim) ρ : e⟨ρ⟩ = e[ρ >> tVar].
+  Proof.
+    substify ; refold.
+    reflexivity.
+  Qed.
 
-Definition swap_var : ren :=
-  1 .: (0 .: (↑ >> ↑)).
+  Definition tip (f : term -> term) : subst :=  (f (tVar 0)).: (↑ >> ids).
 
-Lemma swap_shift2 ρ (t : term) :
-  t⟨swap_var⟩⟨⇑ ⇑ ρ⟩ = t⟨⇑ ⇑ ρ⟩⟨swap_var⟩.
-Proof.
-  unfold swap_var.
-  asimpl ; reflexivity.
-Qed.
+  Lemma tip_shift f t : t⟨↑⟩[tip f] = t⟨↑⟩.
+  Proof.
+    unfold tip.
+    asimpl ; refold.
+    now renamify.
+  Qed.
 
-Lemma swap_shift1 (t u : term) :
-  t⟨swap_var⟩[⇑ (u..)] = t[u⟨↑⟩..].
-Proof.
-  unfold swap_var.
-  substify ; asimpl ; renamify ; refold.
-  now rewrite scons_eta'.
-Qed.
+  Lemma tip_subst (f : term -> term) (t u : term) :
+    (forall σ x, (f x) [σ] = f (x[σ])) ->
+    u[tip f][t ..] = u[(f t)..].
+  Proof.
+    intros Hf.
+    asimpl ; refold.
+    apply ext_term.
+    intros x.
+    unfold tip.
+    asimpl ; cbn ; refold.
+    destruct x ; cbn ; [|easy].
+    rewrite Hf ; now asimpl.
+  Qed.
 
-Lemma swap_subst1 (t u : term) :
-  t⟨swap_var⟩[(u⟨↑⟩ ..)] = t[⇑ (u..)].
-Proof.
-  unfold swap_var.
-  substify ; asimpl ; substify ; reflexivity.
-Qed.
+  Lemma tip_up_ren (f : term -> term) ρ (t : term) :
+    (forall σ x, (f x) [σ] = f (x[σ])) ->
+    t[tip f]⟨⇑ ρ⟩ = t⟨⇑ ρ⟩[tip f].
+  Proof.
+    intros Hf.
+    unfold tip.
+    substify ; asimpl.
+    rewrite Hf ; asimpl.
+    reflexivity.
+  Qed.
+
+  Lemma tip_up_subst (f : term -> term) σ (t : term) :
+    (forall σ' x, (f x) [σ'] = f (x[σ'])) ->
+    t[tip f][⇑ σ] = t[⇑ σ][tip f].
+  Proof.
+    intros Hf.
+    unfold tip.
+    asimpl ; refold.
+    rewrite Hf ; asimpl.
+    now substify.
+  Qed.
+
+  Definition swap_var : ren :=
+    1 .: (0 .: (↑ >> ↑)).
+
+  Lemma swap_up2 ρ (t : term) :
+    t⟨swap_var⟩⟨⇑ ⇑ ρ⟩ = t⟨⇑ ⇑ ρ⟩⟨swap_var⟩.
+  Proof.
+    unfold swap_var.
+    asimpl ; reflexivity.
+  Qed.
+
+  Lemma swap_up1 (t u : term) :
+    t⟨swap_var⟩[⇑ (u..)] = t[u⟨↑⟩..].
+  Proof.
+    unfold swap_var.
+    substify ; asimpl ; renamify ; refold.
+    now rewrite scons_eta'.
+  Qed.
+
+  Lemma swap_subst1 (t u : term) :
+    t⟨swap_var⟩[(u⟨↑⟩ ..)] = t[⇑ (u..)].
+  Proof.
+    unfold swap_var.
+    substify ; asimpl ; substify ; reflexivity.
+  Qed.
+
+End Lemmas.
