code/theories/Theorems.v
@@ -1,0 +1,93 @@
+From Stdlib Require Import Relations Arith Lia Bool List RelationClasses.
+From Interpolation Require Import Utils Syntax Languages Notations Reduction Equations Typing Bidir MetaTheory Interpolation.
+
+(** The most precise result, stated using reduction *)
+Corollary interpolation `{Lang} (A C : type) (t : term) (c : const_split) :
+  ([A] ⊢ t :: C) ->
+  exists B u r l,
+    (forall p, atoms_ty p B ⊆
+      (atoms_ty p A ∪ atoms_const p c.(pconst_l))
+      ∩ (atoms_ty p C ∪ atoms_const (negp p) c.(pconst_r)))
+    /\ (ε,,A ⊢ l :: B) /\ (atoms_tm l ⊆ c.(pconst_l))
+    /\ (ε,,B ⊢ r :: C) /\ (atoms_tm r ⊆ c.(pconst_r))
+    /\ (r[l..] ⤳* u) /\ t ⤳* u.
+Proof.
+  intros Ht.
+  pose proof (normalisation _ _ _ Ht) as (u&?&Hnorm).
+  unshelve eapply interpolation_ind in Hnorm as (B&l&r&Hty&Htm&?&?&?&?).
+  3: exact c.
+  3: exact (split_s split_emp).
+  unfold interpolate_tm, interpolate_ty in * ; cbn in *.
+  exists B, u, r, l.
+  prod_splitter ; try assumption.
+  - intros p b.
+    specialize (Hty p b) ; cbn in *.
+    intuition.
+    now set_solver.
+  - etransitivity ; tea.
+    apply ereflexivity.
+    substify ; asimpl ; refold.
+    eapply term_ext_closed ; tea.
+    intros [|] ? Hin ; cbv in Hin.
+    2: cbv in Hin ; congruence.
+    inversion Hin ; subst.
+    cbn.
+    asimpl ; refold.
+    symmetry.
+    apply subst_id.
+    now intros [|].
+Qed.
+
+(** A “model-theoretic” version, stated with equality with respect to an arbitrary theory *)
+Corollary interpolation_eq `{Theory} (A C : type) (t : term) (c : const_split) :
+  ([A] ⊢ t :: C) ->
+  exists B r l,
+    (forall p, atoms_ty p B ⊆
+      (atoms_ty p A ∪ atoms_const p c.(pconst_l))
+      ∩ (atoms_ty p C ∪ atoms_const (negp p) c.(pconst_r)))
+    /\ (ε,,A ⊢ l :: B) /\ (atoms_tm l ⊆ c.(pconst_l))
+    /\ (ε,,B ⊢ r :: C) /\ (atoms_tm r ⊆ c.(pconst_r))
+    /\ ([A] ⊢ r[l..] ≡ t :: C).
+Proof.
+  intros Ht.
+  epose proof Ht as Ht'.
+  eapply interpolation in Ht' as (B&u&r&l&?&?&?&?&?&?&?).
+  do 3 eexists ; prod_splitter ; eauto.
+  transitivity u.
+  - eauto using subject_reduction_conv with typing.
+  - symmetry.
+    eauto using subject_reduction_conv with typing.
+Qed.
+
+Section Empty.
+  Context `{b : Base}.
+  Existing Instances EmptyLang EmptyTheory.
+
+  (** A simplified version for the empty theory *)
+  Corollary interpolation_empty (A C : type) (t : term) :
+    ([A] ⊢ t :: C) ->
+    exists (B : type) (r l : term),
+      (forall p, (atoms_ty p B) ⊆ (atoms_ty p A) ∩ (atoms_ty p C))
+    /\ (ε,,A ⊢ l :: B) /\ (ε,,B ⊢ r :: C) /\ ([A] ⊢ r[l..] ≡ t :: C).
+  Proof.
+    unshelve eintros (?&?&?&?&?&?&?&?&?)%interpolation_eq.
+    1:{
+      unshelve econstructor ; cbn in *.
+      1-2: exact ⊤.
+      intros [].
+    }
+    cbn in *.
+    do 3 eexists ; prod_splitter ; tea.
+    assert (forall p, atoms_const p ⊤ ≡ ∅).
+    {
+      intros.
+      unfold atoms_const.
+      set_unfold.
+      now intros ? [].
+    }
+    intros.
+    set_solver.
+  Qed.
+
+End Empty.
+  
